module Elaboration.Overloading.Target where

open import Elaboration.Overloading.Common

infixr 5  Æ›_â‡’_
infixl 7  _Â·_
infix  9  `_

data Term : Set where
  lit      : â„• â†’ Term
  flt      : ğ”½ â†’ Term
  `_       : Id â†’ Term
  Æ›_â‡’_     : Id â†’ Term â†’ Term
  _Â·_      : Term â†’ Term â†’ Term
  +        : Term
  +i       : â„• â†’ Term
  +f       : ğ”½ â†’ Term


infix 4 _â‰¤_

data _â‰¤_ : Type â†’ Type â†’ Set where

  s-int :
      Int â‰¤ Int
  s-flt :
      Float â‰¤ Float
  s-arr : âˆ€ {A B C D}
    â†’ C â‰¤ A
    â†’ B â‰¤ D
    â†’ A â‡’ B â‰¤ C â‡’ D
  s-top : âˆ€ {A}
    â†’ A â‰¤ Top
  s-and-l : âˆ€ {A B C}
    â†’ A â‰¤ C
    â†’ A & B â‰¤ C
  s-and-r : âˆ€ {A B C}
    â†’ B â‰¤ C
    â†’ A & B â‰¤ C
  s-and : âˆ€ {A B C}
    â†’ A â‰¤ B
    â†’ A â‰¤ C
    â†’ A â‰¤ B & C

s-refl : âˆ€ {A}
  â†’ A â‰¤ A
s-refl {Top} = s-top
s-refl {Int} = s-int
s-refl {Float} = s-flt
s-refl {A â‡’ Aâ‚} = s-arr s-refl s-refl
s-refl {A & Aâ‚} = s-and (s-and-l s-refl) (s-and-r s-refl)

inv-&-l : âˆ€ {A B C}
  â†’ A â‰¤ B & C
  â†’ A â‰¤ B
inv-&-r : âˆ€ {A B C}
  â†’ A â‰¤ B & C
  â†’ A â‰¤ C

inv-&-l (s-and-l Aâ‰¤BC) = s-and-l (inv-&-l Aâ‰¤BC)
inv-&-l (s-and-r Aâ‰¤BC) = s-and-r (inv-&-l Aâ‰¤BC)
inv-&-l (s-and Aâ‰¤BC Aâ‰¤BCâ‚) = Aâ‰¤BC
inv-&-r (s-and-l Aâ‰¤BC) = s-and-l (inv-&-r Aâ‰¤BC)
inv-&-r (s-and-r Aâ‰¤BC) = s-and-r (inv-&-r Aâ‰¤BC)
inv-&-r (s-and Aâ‰¤BC Aâ‰¤BCâ‚) = Aâ‰¤BCâ‚

â‰¤-trans : âˆ€ {A B C}
  â†’ A â‰¤ B
  â†’ B â‰¤ C
  â†’ A â‰¤ C
â‰¤-trans {B = Top} Aâ‰¤B s-top = Aâ‰¤B
â‰¤-trans {B = Top} Aâ‰¤B (s-and Bâ‰¤C Bâ‰¤Câ‚) = s-and (â‰¤-trans Aâ‰¤B Bâ‰¤C) (â‰¤-trans Aâ‰¤B Bâ‰¤Câ‚)
â‰¤-trans {Int} {Int} x xâ‚ = xâ‚
â‰¤-trans {B = Int} (s-and-l Aâ‰¤B) Bâ‰¤C = s-and-l (â‰¤-trans Aâ‰¤B Bâ‰¤C)
â‰¤-trans {B = Int} (s-and-r Aâ‰¤B) Bâ‰¤C = s-and-r (â‰¤-trans Aâ‰¤B Bâ‰¤C)
â‰¤-trans {Float} {Float} x xâ‚ = xâ‚
â‰¤-trans {B = Float} (s-and-l Aâ‰¤B) Bâ‰¤C = s-and-l (â‰¤-trans Aâ‰¤B Bâ‰¤C)
â‰¤-trans {B = Float} (s-and-r Aâ‰¤B) Bâ‰¤C = s-and-r (â‰¤-trans Aâ‰¤B Bâ‰¤C)
â‰¤-trans {B = B â‡’ Bâ‚} (s-arr Aâ‰¤B Aâ‰¤Bâ‚) (s-arr Bâ‰¤C Bâ‰¤Câ‚) = s-arr (â‰¤-trans Bâ‰¤C Aâ‰¤B) (â‰¤-trans Aâ‰¤Bâ‚ Bâ‰¤Câ‚)
â‰¤-trans {B = B â‡’ Bâ‚} (s-arr Aâ‰¤B Aâ‰¤Bâ‚) s-top = s-top
â‰¤-trans {B = B â‡’ Bâ‚} (s-arr Aâ‰¤B Aâ‰¤Bâ‚) (s-and Bâ‰¤C Bâ‰¤Câ‚) = s-and (â‰¤-trans (s-arr Aâ‰¤B Aâ‰¤Bâ‚) Bâ‰¤C)
                                                               (â‰¤-trans (s-arr Aâ‰¤B Aâ‰¤Bâ‚) Bâ‰¤Câ‚)
â‰¤-trans {B = B â‡’ Bâ‚} (s-and-l Aâ‰¤B) Bâ‰¤C = s-and-l (â‰¤-trans Aâ‰¤B Bâ‰¤C)
â‰¤-trans {B = B â‡’ Bâ‚} (s-and-r Aâ‰¤B) Bâ‰¤C = s-and-r (â‰¤-trans Aâ‰¤B Bâ‰¤C)
â‰¤-trans {B = B & Bâ‚} Aâ‰¤B s-top = s-top
â‰¤-trans {B = B & Bâ‚} Aâ‰¤B (s-and-l Bâ‰¤C) = â‰¤-trans (inv-&-l Aâ‰¤B) Bâ‰¤C
â‰¤-trans {B = B & Bâ‚} Aâ‰¤B (s-and-r Bâ‰¤C) = â‰¤-trans (inv-&-r Aâ‰¤B) Bâ‰¤C
â‰¤-trans {B = B & Bâ‚} Aâ‰¤B (s-and Bâ‰¤C Bâ‰¤Câ‚) = s-and (â‰¤-trans Aâ‰¤B Bâ‰¤C) (â‰¤-trans Aâ‰¤B Bâ‰¤Câ‚)

infix  4  _âŠ¢_â¦‚_

data _âŠ¢_â¦‚_ : Context â†’ Term â†’ Type â†’ Set where

  âŠ¢n : âˆ€ {Î“ n}
    â†’ Î“ âŠ¢ (lit n) â¦‚ Int

  âŠ¢m : âˆ€ {Î“ m}
    â†’ Î“ âŠ¢ (flt m) â¦‚ Float
    
  âŠ¢` : âˆ€ {Î“ x A}
    â†’ Î“ âˆ‹ x â¦‚ A
      -----------
    â†’ Î“ âŠ¢ ` x â¦‚ A
    
  âŠ¢Æ› : âˆ€ {Î“ x N A B}
    â†’ Î“ , x â¦‚ A âŠ¢ N â¦‚ B
      -------------------
    â†’ Î“ âŠ¢ Æ› x â‡’ N â¦‚ A â‡’ B
    
  âŠ¢Â· : âˆ€ {Î“ L M A B}
    â†’ Î“ âŠ¢ L â¦‚ A â‡’ B
    â†’ Î“ âŠ¢ M â¦‚ A
      -------------
    â†’ Î“ âŠ¢ L Â· M â¦‚ B

  âŠ¢& : âˆ€ {Î“ M A B}
    â†’ Î“ âŠ¢ M â¦‚ A
    â†’ Î“ âŠ¢ M â¦‚ B
    â†’ Î“ âŠ¢ M â¦‚ (A & B)

  âŠ¢+ : âˆ€ {Î“}
    â†’ Î“ âŠ¢ + â¦‚ (Int â‡’ Int â‡’ Int) & (Float â‡’ Float â‡’ Float)

  âŠ¢+i : âˆ€ {Î“ n}
    â†’ Î“ âŠ¢ (+i n) â¦‚ Int â‡’ Int

  âŠ¢+f : âˆ€ {Î“ m}
    â†’ Î“ âŠ¢ (+f m) â¦‚ Float â‡’ Float

  âŠ¢sub : âˆ€ {Î“ M A B}
    â†’ Î“ âŠ¢ M â¦‚ A
    â†’ A â‰¤ B
    â†’ Î“ âŠ¢ M â¦‚ B

infix 9 _[_:=_]

_[_:=_] : Term â†’ Id â†’ Term â†’ Term
(` x) [ y := V ] with x â‰Ÿ y
... | yes _         = V
... | no  _         = ` x
(Æ› x â‡’ e) [ y := V ] with x â‰Ÿ y
... | yes _         = Æ› x â‡’ e
... | no  _         = Æ› x â‡’ e [ y := V ]
(eâ‚ Â· eâ‚‚) [ y := V ]  = eâ‚ [ y := V ] Â· eâ‚‚ [ y := V ]
(lit n) [ y := V ]  = lit n
(flt m) [ y := V ]  = flt m
+ [ x := xâ‚ ] = +
+i n [ x := xâ‚ ] = +i n
+f m [ x := xâ‚ ] = +f m

data Value : Term â†’ Set where

  V-n : âˆ€ {n}
    â†’ Value (lit n)

  V-m : âˆ€ {m}
    â†’ Value (flt m)

  V-Æ› : âˆ€ {x e}
    â†’ Value (Æ› x â‡’ e)

  V-+ :
      Value (+)

  V-+i : âˆ€ {n}
    â†’ Value (+i n)

  V-+f : âˆ€ {m}
    â†’ Value (+f m)

infix 4 _â€”â†’_

data _â€”â†’_ : Term â†’ Term â†’ Set where

  Î¾-Â·â‚ : âˆ€ {L Lâ€² M}
    â†’ L â€”â†’ Lâ€²
    â†’ L Â· M â€”â†’ Lâ€² Â· M

  Î¾-Â·â‚‚ : âˆ€ {V M Mâ€²}
    â†’ Value V
    â†’ M â€”â†’ Mâ€²
    â†’ V Â· M â€”â†’ V Â· Mâ€²

  Î²-Æ› : âˆ€ {x N V}
    â†’ Value V
    â†’ (Æ› x â‡’ N) Â· V â€”â†’ N [ x := V ]

  Î²-+-i : âˆ€ {n}
    â†’ + Â· (lit n) â€”â†’ +i n

  Î²-+-f : âˆ€ {m}
    â†’ + Â· (flt m) â€”â†’ +f m

  Î²-+i : âˆ€ {nâ‚ nâ‚‚}
    â†’ (+i nâ‚) Â· (lit nâ‚‚) â€”â†’ (lit (nâ‚ ++n nâ‚‚))

  Î²-+f : âˆ€ {mâ‚ mâ‚‚}
    â†’ (+f mâ‚) Â· (flt mâ‚‚) â€”â†’ (flt (mâ‚ ++f mâ‚‚))

data Progress (M : Term) : Set where

  step : âˆ€ {N}
    â†’ M â€”â†’ N
      ----------
    â†’ Progress M

  done :
      Value M
      ----------
    â†’ Progress M

elim-int : âˆ€ {Î“ n A B C}
  â†’ Î“ âŠ¢ lit n â¦‚ A
  â†’ A â‰¤ B â‡’ C
  â†’ âŠ¥
elim-int (âŠ¢& âŠ¢e âŠ¢eâ‚) (s-and-l Aâ‰¤B) = elim-int âŠ¢e Aâ‰¤B
elim-int (âŠ¢& âŠ¢e âŠ¢eâ‚) (s-and-r Aâ‰¤B) = elim-int âŠ¢eâ‚ Aâ‰¤B
elim-int (âŠ¢sub âŠ¢e x) Aâ‰¤B = elim-int âŠ¢e (â‰¤-trans x Aâ‰¤B)

elim-int' : âˆ€ {Î“ n A B}
  â†’ Î“ âŠ¢ lit n â¦‚ A â‡’ B
  â†’ âŠ¥
elim-int' (âŠ¢sub âŠ¢e x) = elim-int âŠ¢e x

elim-flt : âˆ€ {Î“ n A B C}
  â†’ Î“ âŠ¢ flt n â¦‚ A
  â†’ A â‰¤ B â‡’ C
  â†’ âŠ¥
elim-flt (âŠ¢& âŠ¢e âŠ¢eâ‚) (s-and-l Aâ‰¤B) = elim-flt âŠ¢e Aâ‰¤B
elim-flt (âŠ¢& âŠ¢e âŠ¢eâ‚) (s-and-r Aâ‰¤B) = elim-flt âŠ¢eâ‚ Aâ‰¤B
elim-flt (âŠ¢sub âŠ¢e x) Aâ‰¤B = elim-flt âŠ¢e (â‰¤-trans x Aâ‰¤B)

elim-flt' : âˆ€ {Î“ n A B}
  â†’ Î“ âŠ¢ flt n â¦‚ A â‡’ B
  â†’ âŠ¥
elim-flt' (âŠ¢sub âŠ¢e x) = elim-flt âŠ¢e x

canonical-int : âˆ€ {Î“ M A}
  â†’ Î“ âŠ¢ M â¦‚ A
  â†’ A â‰¤ Int
  â†’ Value M
  â†’ âˆƒ[ n ](M â‰¡ lit n)
canonical-int {A = Int} (âŠ¢n {n = n}) xâ‚ xâ‚‚ = âŸ¨ n , refl âŸ©
canonical-int {A = Int} (âŠ¢sub x xâ‚ƒ) xâ‚ xâ‚‚ = canonical-int x xâ‚ƒ xâ‚‚
canonical-int (âŠ¢& âŠ¢M âŠ¢Mâ‚) (s-and-l Aâ‰¤Int) VM = canonical-int âŠ¢M Aâ‰¤Int VM
canonical-int (âŠ¢sub âŠ¢M x) (s-and-l Aâ‰¤Int) VM = canonical-int âŠ¢M (â‰¤-trans (inv-&-l x) Aâ‰¤Int) VM
canonical-int (âŠ¢& âŠ¢M âŠ¢Mâ‚) (s-and-r Aâ‰¤Int) VM = canonical-int âŠ¢Mâ‚ Aâ‰¤Int VM
canonical-int (âŠ¢sub âŠ¢M x) (s-and-r Aâ‰¤Int) VM = canonical-int âŠ¢M (â‰¤-trans (inv-&-r x) Aâ‰¤Int) VM

canonical-flt : âˆ€ {Î“ M A}
  â†’ Î“ âŠ¢ M â¦‚ A
  â†’ A â‰¤ Float
  â†’ Value M
  â†’ âˆƒ[ m ](M â‰¡ flt m)
canonical-flt (âŠ¢m {m = m}) s-flt VM = âŸ¨ m , refl âŸ©
canonical-flt (âŠ¢sub âŠ¢M x) s-flt VM = canonical-flt âŠ¢M x VM
canonical-flt (âŠ¢& âŠ¢M âŠ¢Mâ‚) (s-and-l Aâ‰¤F) VM = canonical-flt âŠ¢M Aâ‰¤F VM
canonical-flt (âŠ¢sub âŠ¢M x) (s-and-l Aâ‰¤F) VM = canonical-flt âŠ¢M (â‰¤-trans (inv-&-l x) Aâ‰¤F) VM
canonical-flt (âŠ¢& âŠ¢M âŠ¢Mâ‚) (s-and-r Aâ‰¤F) VM = canonical-flt âŠ¢Mâ‚ Aâ‰¤F VM
canonical-flt (âŠ¢sub âŠ¢M x) (s-and-r Aâ‰¤F) VM = canonical-flt âŠ¢M (â‰¤-trans (inv-&-r x) Aâ‰¤F) VM

inv-arr-l : âˆ€ {A B C D}
  â†’ A â‡’ B â‰¤ C â‡’ D
  â†’ C â‰¤ A
inv-arr-r : âˆ€ {A B C D}
  â†’ A â‡’ B â‰¤ C â‡’ D
  â†’ B â‰¤ D
inv-arr-l (s-arr ABâ‰¤CD ABâ‰¤CDâ‚) = ABâ‰¤CD
inv-arr-r (s-arr ABâ‰¤CD ABâ‰¤CDâ‚) = ABâ‰¤CDâ‚

progress-+' : âˆ€ {M T A B}
  â†’ âˆ… âŠ¢ + â¦‚ T
  â†’ T â‰¤ A â‡’ B
  â†’ âˆ… âŠ¢ M â¦‚ A
  â†’ Value M
  â†’ Progress (+ Â· M)
progress-+' (âŠ¢& âŠ¢T âŠ¢Tâ‚) (s-and-l Tâ‰¤AB) âŠ¢M VM = progress-+' âŠ¢T Tâ‰¤AB âŠ¢M VM
progress-+' (âŠ¢& âŠ¢T âŠ¢Tâ‚) (s-and-r Tâ‰¤AB) âŠ¢M VM = progress-+' âŠ¢Tâ‚ Tâ‰¤AB âŠ¢M VM
progress-+' âŠ¢+ (s-and-l (s-arr Tâ‰¤AB Tâ‰¤ABâ‚)) âŠ¢M VM with canonical-int âŠ¢M Tâ‰¤AB VM
... | âŸ¨ n , eq âŸ© rewrite eq = step Î²-+-i
progress-+' âŠ¢+ (s-and-r (s-arr Tâ‰¤AB Tâ‰¤ABâ‚)) âŠ¢M VM with canonical-flt âŠ¢M Tâ‰¤AB VM
... | âŸ¨ m , eq âŸ© rewrite eq = step Î²-+-f
progress-+' (âŠ¢sub âŠ¢T x) ABâ‰¤T âŠ¢M VM = progress-+' âŠ¢T (â‰¤-trans x ABâ‰¤T) âŠ¢M VM

progress-+ : âˆ€ {M A B}
  â†’ âˆ… âŠ¢ + â¦‚ A â‡’ B
  â†’ âˆ… âŠ¢ M â¦‚ A
  â†’ Value M
  â†’ Progress (+ Â· M)
progress-+ (âŠ¢sub âŠ¢N x) âŠ¢M VM = progress-+' âŠ¢N x âŠ¢M VM

progress-+i' : âˆ€ {T M A B n}
  â†’ âˆ… âŠ¢ +i n â¦‚ T
  â†’ T â‰¤ A â‡’ B
  â†’ âˆ… âŠ¢ M â¦‚ A
  â†’ Value M
  â†’ Progress (+i n Â· M)
progress-+i' (âŠ¢& âŠ¢T âŠ¢Tâ‚) (s-and-l Tâ‰¤Aâ‡’B) âŠ¢M VM = progress-+i' âŠ¢T Tâ‰¤Aâ‡’B âŠ¢M VM
progress-+i' (âŠ¢& âŠ¢T âŠ¢Tâ‚) (s-and-r Tâ‰¤Aâ‡’B) âŠ¢M VM = progress-+i' âŠ¢Tâ‚ Tâ‰¤Aâ‡’B âŠ¢M VM
progress-+i' âŠ¢+i (s-arr Tâ‰¤Aâ‡’B Tâ‰¤Aâ‡’Bâ‚) âŠ¢M VM with canonical-int âŠ¢M Tâ‰¤Aâ‡’B VM
... | âŸ¨ n , eq âŸ© rewrite eq = step Î²-+i
progress-+i' (âŠ¢sub âŠ¢T x) Tâ‰¤Aâ‡’B âŠ¢M VM = progress-+i' âŠ¢T (â‰¤-trans x Tâ‰¤Aâ‡’B) âŠ¢M VM

progress-+i : âˆ€ {M A B n}
  â†’ âˆ… âŠ¢ +i n â¦‚ A â‡’ B
  â†’ âˆ… âŠ¢ M â¦‚ A
  â†’ Value M
  â†’ Progress (+i n Â· M)
progress-+i âŠ¢+i âŠ¢M VM with canonical-int âŠ¢M s-int VM
... | âŸ¨ n , eq âŸ© rewrite eq = step Î²-+i
progress-+i (âŠ¢sub âŠ¢N x) âŠ¢M VM = progress-+i' âŠ¢N x âŠ¢M VM

progress-+f' : âˆ€ {T M A B n}
  â†’ âˆ… âŠ¢ +f n â¦‚ T
  â†’ T â‰¤ A â‡’ B
  â†’ âˆ… âŠ¢ M â¦‚ A
  â†’ Value M
  â†’ Progress (+f n Â· M)
progress-+f' (âŠ¢& âŠ¢T âŠ¢Tâ‚) (s-and-l Tâ‰¤Aâ‡’B) âŠ¢M VM = progress-+f' âŠ¢T Tâ‰¤Aâ‡’B âŠ¢M VM
progress-+f' (âŠ¢& âŠ¢T âŠ¢Tâ‚) (s-and-r Tâ‰¤Aâ‡’B) âŠ¢M VM = progress-+f' âŠ¢Tâ‚ Tâ‰¤Aâ‡’B âŠ¢M VM
progress-+f' âŠ¢+f (s-arr Tâ‰¤Aâ‡’B Tâ‰¤Aâ‡’Bâ‚) âŠ¢M VM with canonical-flt âŠ¢M Tâ‰¤Aâ‡’B VM
... | âŸ¨ n , eq âŸ© rewrite eq = step Î²-+f
progress-+f' (âŠ¢sub âŠ¢T x) Tâ‰¤Aâ‡’B âŠ¢M VM = progress-+f' âŠ¢T (â‰¤-trans x Tâ‰¤Aâ‡’B) âŠ¢M VM

progress-+f : âˆ€ {M A B n}
  â†’ âˆ… âŠ¢ +f n â¦‚ A â‡’ B
  â†’ âˆ… âŠ¢ M â¦‚ A
  â†’ Value M
  â†’ Progress (+f n Â· M)
progress-+f âŠ¢+f âŠ¢M VM with canonical-flt âŠ¢M s-flt VM
... | âŸ¨ n , eq âŸ© rewrite eq = step Î²-+f
progress-+f (âŠ¢sub âŠ¢N x) âŠ¢M VM = progress-+f' âŠ¢N x âŠ¢M VM

progress : âˆ€ {e A}
  â†’ âˆ… âŠ¢ e â¦‚ A
  â†’ Progress e
progress âŠ¢n = done V-n
progress âŠ¢m = done V-m
progress (âŠ¢Æ› âŠ¢e) = done V-Æ›
progress (âŠ¢Â· âŠ¢eâ‚ âŠ¢eâ‚‚) with progress âŠ¢eâ‚ | progress âŠ¢eâ‚‚
... | step sâ‚ | _ = step (Î¾-Â·â‚ sâ‚)
... | done vâ‚ | step sâ‚‚ = step (Î¾-Â·â‚‚ vâ‚ sâ‚‚)
... | done V-n | done vâ‚‚ = âŠ¥-elim (elim-int' âŠ¢eâ‚)
... | done V-m | done vâ‚‚ = âŠ¥-elim (elim-flt' âŠ¢eâ‚)
... | done V-Æ› | done vâ‚‚ = step (Î²-Æ› vâ‚‚)
... | done V-+ | done vâ‚‚ = progress-+ âŠ¢eâ‚ âŠ¢eâ‚‚ vâ‚‚
... | done V-+i | done vâ‚‚ = progress-+i âŠ¢eâ‚ âŠ¢eâ‚‚ vâ‚‚
... | done V-+f | done vâ‚‚ = progress-+f âŠ¢eâ‚ âŠ¢eâ‚‚ vâ‚‚
progress (âŠ¢& âŠ¢e âŠ¢eâ‚) = progress âŠ¢e
progress âŠ¢+ = done V-+
progress âŠ¢+i = done V-+i
progress âŠ¢+f = done V-+f
progress (âŠ¢sub âŠ¢e x) = progress âŠ¢e

ext : âˆ€ {Î“ Î”}
  â†’ (âˆ€ {x A}     â†’         Î“ âˆ‹ x â¦‚ A â†’         Î” âˆ‹ x â¦‚ A)
    -----------------------------------------------------
  â†’ (âˆ€ {x y A B} â†’ Î“ , y â¦‚ B âˆ‹ x â¦‚ A â†’ Î” , y â¦‚ B âˆ‹ x â¦‚ A)
ext Ï Z           =  Z
ext Ï (S xâ‰¢y âˆ‹x)  =  S xâ‰¢y (Ï âˆ‹x)

rename : âˆ€ {Î“ Î”}
  â†’ (âˆ€ {x A} â†’ Î“ âˆ‹ x â¦‚ A â†’ Î” âˆ‹ x â¦‚ A)
    ----------------------------------
  â†’ (âˆ€ {M A} â†’ Î“ âŠ¢ M â¦‚ A â†’ Î” âŠ¢ M â¦‚ A)
rename Ï âŠ¢n = âŠ¢n
rename Ï âŠ¢m = âŠ¢m
rename Ï (âŠ¢` âˆ‹w)    =  âŠ¢` (Ï âˆ‹w)
rename Ï (âŠ¢Æ› âŠ¢N)    =  âŠ¢Æ› (rename (ext Ï) âŠ¢N)
rename Ï (âŠ¢Â· âŠ¢L âŠ¢M) =  âŠ¢Â· (rename Ï âŠ¢L) (rename Ï âŠ¢M)
rename Ï (âŠ¢& âŠ¢L âŠ¢M) =  âŠ¢& (rename Ï âŠ¢L) (rename Ï âŠ¢M)
rename Ï (âŠ¢sub âŠ¢L s) = âŠ¢sub (rename Ï âŠ¢L) s
rename Ï âŠ¢+ = âŠ¢+
rename Ï âŠ¢+i = âŠ¢+i
rename Ï âŠ¢+f = âŠ¢+f

weaken : âˆ€ {Î“ M A}
  â†’ âˆ… âŠ¢ M â¦‚ A
    ----------
  â†’ Î“ âŠ¢ M â¦‚ A
weaken {Î“} âŠ¢M = rename Ï âŠ¢M
  where
  Ï : âˆ€ {z C}
    â†’ âˆ… âˆ‹ z â¦‚ C
      ---------
    â†’ Î“ âˆ‹ z â¦‚ C
  Ï ()

drop : âˆ€ {Î“ x M A B C}
  â†’ Î“ , x â¦‚ A , x â¦‚ B âŠ¢ M â¦‚ C
    --------------------------
  â†’ Î“ , x â¦‚ B âŠ¢ M â¦‚ C
drop {Î“} {x} {M} {A} {B} {C} âŠ¢M = rename Ï âŠ¢M
  where
  Ï : âˆ€ {z C}
    â†’ Î“ , x â¦‚ A , x â¦‚ B âˆ‹ z â¦‚ C
      -------------------------
    â†’ Î“ , x â¦‚ B âˆ‹ z â¦‚ C
  Ï Z                 =  Z
  Ï (S xâ‰¢x Z)         =  âŠ¥-elim (xâ‰¢x refl)
  Ï (S zâ‰¢x (S _ âˆ‹z))  =  S zâ‰¢x âˆ‹z

swap : âˆ€ {Î“ x y M A B C}
  â†’ x â‰¢ y
  â†’ Î“ , y â¦‚ B , x â¦‚ A âŠ¢ M â¦‚ C
    --------------------------
  â†’ Î“ , x â¦‚ A , y â¦‚ B âŠ¢ M â¦‚ C
swap {Î“} {x} {y} {M} {A} {B} {C} xâ‰¢y âŠ¢M = rename Ï âŠ¢M
  where
  Ï : âˆ€ {z C}
    â†’ Î“ , y â¦‚ B , x â¦‚ A âˆ‹ z â¦‚ C
      --------------------------
    â†’ Î“ , x â¦‚ A , y â¦‚ B âˆ‹ z â¦‚ C
  Ï Z                   =  S xâ‰¢y Z
  Ï (S zâ‰¢x Z)           =  Z
  Ï (S zâ‰¢x (S zâ‰¢y âˆ‹z))  =  S zâ‰¢y (S zâ‰¢x âˆ‹z)

subst : âˆ€ {Î“ x N V A B}
  â†’ âˆ… âŠ¢ V â¦‚ A
  â†’ Î“ , x â¦‚ A âŠ¢ N â¦‚ B
    --------------------
  â†’ Î“ âŠ¢ N [ x := V ] â¦‚ B
subst {x = y} âŠ¢V âŠ¢n = âŠ¢n
subst {x = y} âŠ¢V âŠ¢m = âŠ¢m
subst {x = y} âŠ¢V (âŠ¢` {x = x} Z) with x â‰Ÿ y
... | yes _         =  weaken âŠ¢V
... | no  xâ‰¢y       =  âŠ¥-elim (xâ‰¢y refl)
subst {x = y} âŠ¢V (âŠ¢` {x = x} (S xâ‰¢y âˆ‹x)) with x â‰Ÿ y
... | yes refl      =  âŠ¥-elim (xâ‰¢y refl)
... | no  _         =  âŠ¢` âˆ‹x
subst {x = y} âŠ¢V (âŠ¢Æ› {x = x} âŠ¢N) with x â‰Ÿ y
... | yes refl      =  âŠ¢Æ› (drop âŠ¢N)
... | no  xâ‰¢y       =  âŠ¢Æ› (subst âŠ¢V (swap xâ‰¢y âŠ¢N))
subst âŠ¢V (âŠ¢Â· âŠ¢L âŠ¢M) = âŠ¢Â· (subst âŠ¢V âŠ¢L) (subst âŠ¢V âŠ¢M)
subst âŠ¢V (âŠ¢& âŠ¢L âŠ¢M) = âŠ¢& (subst âŠ¢V âŠ¢L) (subst âŠ¢V âŠ¢M)
subst âŠ¢V (âŠ¢sub âŠ¢L s) = âŠ¢sub (subst âŠ¢V âŠ¢L) s
subst âŠ¢V âŠ¢+ = âŠ¢+
subst âŠ¢V âŠ¢+i = âŠ¢+i
subst âŠ¢V âŠ¢+f = âŠ¢+f

inv-lam' : âˆ€ {Î“ x e A B T}
  â†’ Î“ âŠ¢ Æ› x â‡’ e â¦‚ T
  â†’ T â‰¤ A â‡’ B
  â†’ âˆƒ[ A' ]( âˆƒ[ B' ] ((Î“ , x â¦‚ A' âŠ¢ e â¦‚ B') Ã— (A â‰¤ A') Ã— (B' â‰¤ B)))
inv-lam' (âŠ¢Æ› {A = A} {B} âŠ¢e) (s-arr Tâ‰¤AB Tâ‰¤ABâ‚) = âŸ¨ A , âŸ¨ B , âŸ¨ âŠ¢e , âŸ¨ Tâ‰¤AB , Tâ‰¤ABâ‚ âŸ© âŸ© âŸ© âŸ©
inv-lam' (âŠ¢sub âŠ¢e x) (s-arr Tâ‰¤AB Tâ‰¤ABâ‚) = inv-lam' âŠ¢e (â‰¤-trans x (s-arr Tâ‰¤AB Tâ‰¤ABâ‚))
inv-lam' (âŠ¢& âŠ¢e âŠ¢eâ‚) (s-and-l Tâ‰¤AB) = inv-lam' âŠ¢e Tâ‰¤AB
inv-lam' (âŠ¢sub âŠ¢e x) (s-and-l Tâ‰¤AB) = inv-lam' âŠ¢e (â‰¤-trans (inv-&-l x) Tâ‰¤AB)
inv-lam' (âŠ¢& âŠ¢e âŠ¢eâ‚) (s-and-r Tâ‰¤AB) = inv-lam' âŠ¢eâ‚ Tâ‰¤AB
inv-lam' (âŠ¢sub âŠ¢e x) (s-and-r Tâ‰¤AB) = inv-lam' âŠ¢e (â‰¤-trans (inv-&-r x) Tâ‰¤AB)

inv-lam : âˆ€ {Î“ x e A B}
  â†’ Î“ âŠ¢ Æ› x â‡’ e â¦‚ A â‡’ B
  â†’ âˆƒ[ A' ]( âˆƒ[ B' ] ((Î“ , x â¦‚ A' âŠ¢ e â¦‚ B') Ã— (A â‰¤ A') Ã— (B' â‰¤ B)))
inv-lam {A = A} {B = B} (âŠ¢Æ› âŠ¢e) = âŸ¨ A , âŸ¨ B , âŸ¨ âŠ¢e , âŸ¨ s-refl , s-refl âŸ© âŸ© âŸ© âŸ©
inv-lam {A = A} {B = B} (âŠ¢sub âŠ¢e x) = inv-lam' âŠ¢e x

inv-int : âˆ€ {Î“ n A}
  â†’ Î“ âŠ¢ lit n â¦‚ A
  â†’ Int â‰¤ A
inv-int âŠ¢n = s-refl
inv-int (âŠ¢& âŠ¢e âŠ¢eâ‚) = s-and (inv-int âŠ¢e) (inv-int âŠ¢eâ‚)
inv-int (âŠ¢sub âŠ¢e x) = â‰¤-trans (inv-int âŠ¢e) x

inv-flt : âˆ€ {Î“ m A}
  â†’ Î“ âŠ¢ flt m â¦‚ A
  â†’ Float â‰¤ A
inv-flt âŠ¢m = s-flt
inv-flt (âŠ¢& âŠ¢M âŠ¢Mâ‚) = s-and (inv-flt âŠ¢M) (inv-flt âŠ¢Mâ‚)
inv-flt (âŠ¢sub âŠ¢M x) = â‰¤-trans (inv-flt âŠ¢M) x

Â¬Intâ‰¤Float : Int â‰¤ Float â†’ âŠ¥
Â¬Intâ‰¤Float ()

Â¬Floatâ‰¤Int : Float â‰¤ Int â†’ âŠ¥
Â¬Floatâ‰¤Int ()

inv-+-i+' : âˆ€ {Î“ T A B}
  â†’ Î“ âŠ¢ + â¦‚ T
  â†’ T â‰¤ A â‡’ B
  â†’ Int â‰¤ A
  â†’ Int â‡’ Int â‰¤ B
inv-+-i+' (âŠ¢& âŠ¢T âŠ¢Tâ‚) (s-and-l Tâ‰¤AB) Intâ‰¤A = inv-+-i+' âŠ¢T Tâ‰¤AB Intâ‰¤A
inv-+-i+' (âŠ¢& âŠ¢T âŠ¢Tâ‚) (s-and-r Tâ‰¤AB) Intâ‰¤A = inv-+-i+' âŠ¢Tâ‚ Tâ‰¤AB Intâ‰¤A
inv-+-i+' âŠ¢+ (s-and-l (s-arr Tâ‰¤AB Tâ‰¤ABâ‚)) Intâ‰¤A = Tâ‰¤ABâ‚
inv-+-i+' âŠ¢+ (s-and-r (s-arr Tâ‰¤AB Tâ‰¤ABâ‚)) Intâ‰¤A = âŠ¥-elim (Â¬Intâ‰¤Float (â‰¤-trans Intâ‰¤A Tâ‰¤AB))
inv-+-i+' (âŠ¢sub âŠ¢T x) Tâ‰¤AB Intâ‰¤A = inv-+-i+' âŠ¢T (â‰¤-trans x Tâ‰¤AB) Intâ‰¤A

inv-+-i+ : âˆ€ {Î“ A B}
  â†’ Î“ âŠ¢ + â¦‚ A â‡’ B
  â†’ Int â‰¤ A
  â†’ Int â‡’ Int â‰¤ B
inv-+-i+ (âŠ¢sub âŠ¢M x) Intâ‰¤A = inv-+-i+' âŠ¢M x Intâ‰¤A

inv-+-f+' : âˆ€ {Î“ T A B}
  â†’ Î“ âŠ¢ + â¦‚ T
  â†’ T â‰¤ A â‡’ B
  â†’ Float â‰¤ A
  â†’ Float â‡’ Float â‰¤ B
inv-+-f+' (âŠ¢& âŠ¢T âŠ¢Tâ‚) (s-and-l Tâ‰¤AB) Intâ‰¤A = inv-+-f+' âŠ¢T Tâ‰¤AB Intâ‰¤A
inv-+-f+' (âŠ¢& âŠ¢T âŠ¢Tâ‚) (s-and-r Tâ‰¤AB) Intâ‰¤A = inv-+-f+' âŠ¢Tâ‚ Tâ‰¤AB Intâ‰¤A
inv-+-f+' âŠ¢+ (s-and-l (s-arr Tâ‰¤AB Tâ‰¤ABâ‚)) Intâ‰¤A = âŠ¥-elim (Â¬Floatâ‰¤Int (â‰¤-trans Intâ‰¤A Tâ‰¤AB))
inv-+-f+' âŠ¢+ (s-and-r (s-arr Tâ‰¤AB Tâ‰¤ABâ‚)) Intâ‰¤A = Tâ‰¤ABâ‚
inv-+-f+' (âŠ¢sub âŠ¢T x) Tâ‰¤AB Intâ‰¤A = inv-+-f+' âŠ¢T (â‰¤-trans x Tâ‰¤AB) Intâ‰¤A

inv-+-f+ : âˆ€ {Î“ A B}
  â†’ Î“ âŠ¢ + â¦‚ A â‡’ B
  â†’ Float â‰¤ A
  â†’ Float â‡’ Float â‰¤ B
inv-+-f+ (âŠ¢sub âŠ¢M x) Intâ‰¤A = inv-+-f+' âŠ¢M x Intâ‰¤A

inv-+i' : âˆ€ {n A B T}
  â†’ âˆ… âŠ¢ +i n â¦‚ T
  â†’ T â‰¤ A â‡’ B
  â†’ Int â‰¤ B
inv-+i' (âŠ¢& âŠ¢M âŠ¢Mâ‚) (s-and-l Tâ‰¤AB) = inv-+i' âŠ¢M Tâ‰¤AB
inv-+i' (âŠ¢& âŠ¢M âŠ¢Mâ‚) (s-and-r Tâ‰¤AB) = inv-+i' âŠ¢Mâ‚ Tâ‰¤AB
inv-+i' âŠ¢+i (s-arr Tâ‰¤AB Tâ‰¤ABâ‚) = Tâ‰¤ABâ‚
inv-+i' (âŠ¢sub âŠ¢M x) Tâ‰¤AB = inv-+i' âŠ¢M (â‰¤-trans x Tâ‰¤AB)

inv-+i : âˆ€ {n A B}
  â†’ âˆ… âŠ¢ +i n â¦‚ A â‡’ B
  â†’ Int â‰¤ B
inv-+i âŠ¢+i = s-int
inv-+i (âŠ¢sub âŠ¢e x) = inv-+i' âŠ¢e x

inv-+f' : âˆ€ {m A B T}
  â†’ âˆ… âŠ¢ +f m â¦‚ T
  â†’ T â‰¤ A â‡’ B
  â†’ Float â‰¤ B
inv-+f' (âŠ¢& âŠ¢M âŠ¢Mâ‚) (s-and-l Tâ‰¤AB) = inv-+f' âŠ¢M Tâ‰¤AB
inv-+f' (âŠ¢& âŠ¢M âŠ¢Mâ‚) (s-and-r Tâ‰¤AB) = inv-+f' âŠ¢Mâ‚ Tâ‰¤AB
inv-+f' âŠ¢+f (s-arr Tâ‰¤AB Tâ‰¤ABâ‚) = Tâ‰¤ABâ‚
inv-+f' (âŠ¢sub âŠ¢M x) Tâ‰¤AB = inv-+f' âŠ¢M (â‰¤-trans x Tâ‰¤AB)

inv-+f : âˆ€ {m A B}
  â†’ âˆ… âŠ¢ +f m â¦‚ A â‡’ B
  â†’ Float â‰¤ B
inv-+f âŠ¢+f = s-flt
inv-+f (âŠ¢sub âŠ¢M x) = inv-+f' âŠ¢M x
  

preserve : âˆ€ {M N A}
  â†’ âˆ… âŠ¢ M â¦‚ A
  â†’ M â€”â†’ N
    ----------
  â†’ âˆ… âŠ¢ N â¦‚ A
preserve (âŠ¢Â· âŠ¢e âŠ¢eâ‚) (Î¾-Â·â‚ Mâ†’N) = âŠ¢Â· (preserve âŠ¢e Mâ†’N) âŠ¢eâ‚
preserve (âŠ¢Â· âŠ¢e âŠ¢eâ‚) (Î¾-Â·â‚‚ x Mâ†’N) = âŠ¢Â· âŠ¢e (preserve âŠ¢eâ‚ Mâ†’N)
preserve (âŠ¢Â· âŠ¢e âŠ¢eâ‚) (Î²-Æ› x) with inv-lam âŠ¢e
... | âŸ¨ A' , âŸ¨ B' , âŸ¨ âŠ¢e' , âŸ¨ Aâ‰¤A' , B'â‰¤B âŸ© âŸ© âŸ© âŸ© = subst (âŠ¢sub âŠ¢eâ‚ Aâ‰¤A') (âŠ¢sub âŠ¢e' B'â‰¤B)
preserve (âŠ¢Â· âŠ¢e âŠ¢eâ‚) Î²-+-i = âŠ¢sub âŠ¢+i (inv-+-i+ âŠ¢e (inv-int âŠ¢eâ‚))
preserve (âŠ¢Â· âŠ¢e âŠ¢eâ‚) Î²-+-f = âŠ¢sub âŠ¢+f (inv-+-f+ âŠ¢e (inv-flt âŠ¢eâ‚))
preserve (âŠ¢Â· âŠ¢e âŠ¢eâ‚) Î²-+i = âŠ¢sub âŠ¢n (inv-+i âŠ¢e)
preserve (âŠ¢Â· âŠ¢e âŠ¢eâ‚) Î²-+f = âŠ¢sub âŠ¢m (inv-+f âŠ¢e)
preserve (âŠ¢& âŠ¢e âŠ¢eâ‚) Mâ†’N = âŠ¢& (preserve âŠ¢e Mâ†’N) (preserve âŠ¢eâ‚ Mâ†’N)
preserve (âŠ¢sub âŠ¢e x) Mâ†’N = âŠ¢sub (preserve âŠ¢e Mâ†’N) x
