{-# OPTIONS --allow-unsolved-metas #-}
module Record.Algo.Properties where

open import Record.Prelude hiding (_â‰¤?_) renaming (_â‰¤_ to _â‰¤n_)
open import Record.Common
open import Record.Properties
open import Record.Algo

----------------------------------------------------------------------
--                                                                  --
--                            Subtyping                             --
--                                                                  --
----------------------------------------------------------------------

{-
-- inversion lemmas

â‰¤a-hint-invâ‚ : âˆ€ {Î“ H A B e}
  â†’ Î“ âŠ¢a A â‡’ B â‰¤ âŸ¦ e âŸ§â‡’ H
  â†’ âˆƒ[ C ] Î“ âŠ¢a Ï„ A â‡› e â‡› C
â‰¤a-hint-invâ‚ (â‰¤a-hint {C = C} x â‰¤a) = âŸ¨ C , x âŸ©

â‰¤a-hint-invâ‚‚ : âˆ€ {Î“ H A B e}
  â†’ Î“ âŠ¢a A â‡’ B â‰¤ âŸ¦ e âŸ§â‡’ H
  â†’ Î“ âŠ¢a B â‰¤ H
â‰¤a-hint-invâ‚‚ (â‰¤a-hint x â‰¤) = â‰¤
-}

{-
-- this lemma is obviously wrong

â‰¤a-refl-Ï„ : âˆ€ {Î“ A B C}
  â†’ Î“ âŠ¢a B â‰¤ Ï„ A â‡ C
  â†’ A â‰¢ Top
  â†’ C â‰¡ A
â‰¤a-refl-Ï„ â‰¤a-int neq = refl
â‰¤a-refl-Ï„ â‰¤a-base neq = refl
â‰¤a-refl-Ï„ â‰¤a-top neq = âŠ¥-elim (neq refl)
â‰¤a-refl-Ï„ (â‰¤a-arr Bâ‰¤A Bâ‰¤Aâ‚) neq = {!!}
â‰¤a-refl-Ï„ (â‰¤a-and-l Bâ‰¤A) neq = â‰¤a-refl-Ï„ Bâ‰¤A neq
â‰¤a-refl-Ï„ (â‰¤a-and-r Bâ‰¤A) neq = â‰¤a-refl-Ï„ Bâ‰¤A neq
â‰¤a-refl-Ï„ (â‰¤a-and Bâ‰¤A Bâ‰¤Aâ‚) neq = {!!}

âŠ¢a-refl : âˆ€ {Î“ A B e}
  â†’ Î“ âŠ¢a Ï„ A â‡› e â‡› B
  â†’ A â‰¢ Top
  â†’ B â‰¡ A
âŠ¢a-refl âŠ¢a-lit neq = âŠ¥-elim (neq refl)
âŠ¢a-refl (âŠ¢a-var x) neq =  âŠ¥-elim (neq refl)
âŠ¢a-refl (âŠ¢a-app âŠ¢e) neq = {!!}
âŠ¢a-refl (âŠ¢a-ann âŠ¢e) neq =  âŠ¥-elim (neq refl)
âŠ¢a-refl (âŠ¢a-lamâ‚ âŠ¢e) neq = {!âŠ¢a-refl âŠ¢e!} -- A -> Top
âŠ¢a-refl (âŠ¢a-lamâ‚ƒ âŠ¢e âŠ¢eâ‚) neq = {!âŠ¢a-refl âŠ¢eâ‚!} -- Top & Top
âŠ¢a-refl (âŠ¢a-sub x âŠ¢e xâ‚) neq = â‰¤a-refl-Ï„ xâ‚ neq

-}

----------------------------------------------------------------------
--+                                                                +--
--+                             Shift                              +--
--+                                                                +--
----------------------------------------------------------------------

â‡§-â‡§-comm : âˆ€ H m n
  â†’ m â‰¤n n
  â†’ H â‡§ m â‡§ suc n â‰¡ H â‡§ n â‡§ m
â‡§-â‡§-comm â–¡ m n mâ‰¤n = refl
â‡§-â‡§-comm (Ï„ A) m n mâ‰¤n = refl
â‡§-â‡§-comm (âŸ¦ e âŸ§â‡’ H) m n mâ‰¤n rewrite â†‘-â†‘-comm e m n mâ‰¤n | â‡§-â‡§-comm H m n mâ‰¤n = refl
â‡§-â‡§-comm (âŒŠ xâ‚ âŒ‹â‡’ H) m n x = {!!}

â‡§-â‡©-id : âˆ€ H n
  â†’ H â‡§ n â‡© n â‰¡ H
â‡§-â‡©-id â–¡ n = refl  
â‡§-â‡©-id (Ï„ A) n = refl
â‡§-â‡©-id (âŸ¦ e âŸ§â‡’ H) n rewrite â†‘-â†“-id e n | â‡§-â‡©-id H n = refl
â‡§-â‡©-id (âŒŠ l âŒ‹â‡’ H) n rewrite â‡§-â‡©-id H n = refl


infix 4 _~â‡§~_
data _~â‡§~_ : Hint â†’ â„• â†’ Set where

  sdh-â–¡ : âˆ€ {n}
    â†’ â–¡ ~â‡§~ n

  sdh-Ï„ : âˆ€ {n A}
    â†’ (Ï„ A) ~â‡§~ n

  sdh-h : âˆ€ {n e H}
    â†’ e ~â†‘~ n
    â†’ H ~â‡§~ n
    â†’ (âŸ¦ e âŸ§â‡’ H) ~â‡§~ n

  sdh-l : âˆ€ {n l H}
    â†’ H ~â‡§~ n
    â†’ (âŒŠ l âŒ‹â‡’ H) ~â‡§~ n

â‡§-shiftedh : âˆ€ {H n}
  â†’ (H â‡§ n) ~â‡§~ n
â‡§-shiftedh {â–¡} = sdh-â–¡  
â‡§-shiftedh {Ï„ A} = sdh-Ï„
â‡§-shiftedh {âŸ¦ e âŸ§â‡’ H} = sdh-h â†‘-shifted â‡§-shiftedh
â‡§-shiftedh {âŒŠ l âŒ‹â‡’ H} = sdh-l â‡§-shiftedh

â‡§-shiftedh-n : âˆ€ {H m n}
  â†’ m â‰¤n suc n
  â†’ H ~â‡§~ n
  â†’ (H â‡§ m) ~â‡§~ suc n
â‡§-shiftedh-n {â–¡} mâ‰¤n sdh = sdh-â–¡
â‡§-shiftedh-n {Ï„ A} mâ‰¤n sdh = sdh-Ï„
â‡§-shiftedh-n {âŸ¦ e âŸ§â‡’ H} mâ‰¤n (sdh-h sd sdh) = sdh-h (â†‘-shifted-n mâ‰¤n sd) (â‡§-shiftedh-n mâ‰¤n sdh)
â‡§-shiftedh-n {âŒŠ l âŒ‹â‡’ H} mâ‰¤n (sdh-l sd) = sdh-l (â‡§-shiftedh-n mâ‰¤n sd)

â‡©-â‡§-comm : âˆ€ H m n
  â†’ m â‰¤n n
  â†’ H ~â‡§~ n
  â†’ H â‡© n â‡§ m â‰¡ H â‡§ m â‡© (suc n)
â‡©-â‡§-comm â–¡ m n mâ‰¤n sdh = refl
â‡©-â‡§-comm (Ï„ A) m n mâ‰¤n sdh = refl
â‡©-â‡§-comm (âŸ¦ e âŸ§â‡’ H) m n mâ‰¤n (sdh-h sd sdh) rewrite â†“-â†‘-comm e m n mâ‰¤n sd rewrite â‡©-â‡§-comm H m n mâ‰¤n sdh = refl
â‡©-â‡§-comm (âŒŠ l âŒ‹â‡’ H) m n mâ‰¤n (sdh-l sd) rewrite â‡©-â‡§-comm H m n mâ‰¤n sd = refl

Hâ‰¢â–¡-â‡© : âˆ€ {H n}
  â†’ H â‰¢ â–¡
  â†’ H â‡© n â‰¢ â–¡
Hâ‰¢â–¡-â‡© {â–¡} Hâ‰¢â–¡ = Hâ‰¢â–¡
Hâ‰¢â–¡-â‡© {Ï„ x} Hâ‰¢â–¡ = Hâ‰¢â–¡
Hâ‰¢â–¡-â‡© {âŸ¦ x âŸ§â‡’ H} Hâ‰¢â–¡ = Î» ()

Hâ‰¢â–¡-â‡§ : âˆ€ {H n}
  â†’ H â‰¢ â–¡
  â†’ H â‡§ n â‰¢ â–¡
Hâ‰¢â–¡-â‡§ {â–¡} Hâ‰¢â–¡ = Hâ‰¢â–¡
Hâ‰¢â–¡-â‡§ {Ï„ x} Hâ‰¢â–¡ = Hâ‰¢â–¡
Hâ‰¢â–¡-â‡§ {âŸ¦ x âŸ§â‡’ H} Hâ‰¢â–¡ = Î» ()

----------------------------------------------------------------------
--+                                                                +--
--+                           Weakening                            +--
--+                                                                +--
----------------------------------------------------------------------

â‰¤a-weaken : âˆ€ {Î“ A B C H n nâ‰¤l}
  â†’ Î“ âŠ¢a B â‰¤ H â‡ C
  â†’ Î“ â†‘ n [ nâ‰¤l ] A âŠ¢a B â‰¤ (H â‡§ n) â‡ C

âŠ¢a-weaken : âˆ€ {Î“ e H A B n nâ‰¤l}
  â†’ Î“ âŠ¢a H â‡› e â‡› B
  â†’ Î“ â†‘ n [ nâ‰¤l ] A âŠ¢a H â‡§ n â‡› e â†‘ n â‡› B

â‰¤a-weaken â‰¤a-int = â‰¤a-int
â‰¤a-weaken â‰¤a-base = â‰¤a-base
â‰¤a-weaken â‰¤a-top = â‰¤a-top
â‰¤a-weaken â‰¤a-â–¡ = â‰¤a-â–¡
â‰¤a-weaken (â‰¤a-arr Câ‰¤A Bâ‰¤D) = â‰¤a-arr (â‰¤a-weaken Câ‰¤A) (â‰¤a-weaken Bâ‰¤D)
â‰¤a-weaken (â‰¤a-hint âŠ¢e Bâ‰¤H) = â‰¤a-hint (âŠ¢a-weaken âŠ¢e) (â‰¤a-weaken Bâ‰¤H)
â‰¤a-weaken (â‰¤a-and-l â‰¤ Hâ‰¢â–¡) = â‰¤a-and-l (â‰¤a-weaken â‰¤) (Hâ‰¢â–¡-â‡§ Hâ‰¢â–¡)
â‰¤a-weaken (â‰¤a-and-r â‰¤ Hâ‰¢â–¡) = â‰¤a-and-r (â‰¤a-weaken â‰¤) (Hâ‰¢â–¡-â‡§ Hâ‰¢â–¡)
â‰¤a-weaken (â‰¤a-and â‰¤â‚ â‰¤â‚‚) = â‰¤a-and (â‰¤a-weaken â‰¤â‚) (â‰¤a-weaken â‰¤â‚‚)
â‰¤a-weaken (â‰¤a-rcd x) = {!!}
â‰¤a-weaken (â‰¤a-hint-l x) = {!!}

â‰¤a-weaken-0 : âˆ€ {Î“ A B H C}
  â†’ Î“ âŠ¢a B â‰¤ H â‡ C
  â†’ Î“ , A âŠ¢a B â‰¤ (H â‡§ 0) â‡ C
â‰¤a-weaken-0 Bâ‰¤H = â‰¤a-weaken {nâ‰¤l = zâ‰¤n} Bâ‰¤H  

â‡§-â‡§-comm-0 : âˆ€ H n
  â†’ H â‡§ n â‡§ 0 â‰¡ H â‡§ 0 â‡§ (suc n)
â‡§-â‡§-comm-0 H n rewrite â‡§-â‡§-comm H 0 n zâ‰¤n = refl

âŠ¢a-weaken âŠ¢a-lit = âŠ¢a-lit
âŠ¢a-weaken {nâ‰¤l = nâ‰¤l} (âŠ¢a-var xâˆˆÎ“) = âŠ¢a-var (âˆ‹-weaken xâˆˆÎ“ nâ‰¤l)
âŠ¢a-weaken (âŠ¢a-app âŠ¢e) = âŠ¢a-app (âŠ¢a-weaken âŠ¢e)
âŠ¢a-weaken (âŠ¢a-ann âŠ¢e) = âŠ¢a-ann (âŠ¢a-weaken âŠ¢e)
âŠ¢a-weaken {nâ‰¤l = nâ‰¤l} (âŠ¢a-lamâ‚ âŠ¢e) = âŠ¢a-lamâ‚ (âŠ¢a-weaken {nâ‰¤l = sâ‰¤s nâ‰¤l} âŠ¢e)
âŠ¢a-weaken {H = âŸ¦ _ âŸ§â‡’ H} {A = A} {n = n} {nâ‰¤l = nâ‰¤l} (âŠ¢a-lamâ‚‚ âŠ¢e âŠ¢f) with âŠ¢a-weaken {A = A} {n = suc n} {nâ‰¤l = sâ‰¤s nâ‰¤l} âŠ¢f
... | ind-f rewrite sym (â‡§-â‡§-comm-0 H n) = âŠ¢a-lamâ‚‚ (âŠ¢a-weaken âŠ¢e) ind-f
âŠ¢a-weaken (âŠ¢a-sub pv âŠ¢e Bâ‰¤H) = âŠ¢a-sub (â†‘-pv-prv pv) (âŠ¢a-weaken âŠ¢e) (â‰¤a-weaken Bâ‰¤H)
âŠ¢a-weaken (âŠ¢a-& âŠ¢eâ‚ âŠ¢eâ‚‚) = âŠ¢a-& (âŠ¢a-weaken âŠ¢eâ‚) (âŠ¢a-weaken âŠ¢eâ‚‚)
âŠ¢a-weaken {e = ğ•£ x} (âŠ¢a-rcd xâ‚) = {!!}
âŠ¢a-weaken {e = e ğ•¡ x} (âŠ¢a-prj xâ‚) = {!!}

up : â„• â†’ Apps â†’ Apps
up n [] = []
up n (e âˆ·a as) = (e â†‘ n) âˆ·a (up n as)
up n (l âˆ·l as) = l âˆ·l (up n as)

spl-weaken : âˆ€ {H A es T As A' n}
  â†’ âŸ¦ H , A âŸ§â†’âŸ¦ es , T , As , A' âŸ§
  â†’ âŸ¦ H â‡§ n , A âŸ§â†’âŸ¦ up n es , T , As , A' âŸ§
spl-weaken none-â–¡ = none-â–¡
spl-weaken none-Ï„ = none-Ï„
spl-weaken (have-a spl) = have-a (spl-weaken spl)
spl-weaken (have-l spl) = have-l (spl-weaken spl)

----------------------------------------------------------------------
--+                                                                +--
--+                         Strengthening                          +--
--+                                                                +--
----------------------------------------------------------------------


â‰¤a-strengthen : âˆ€ {Î“ A B H n}
  â†’ Î“ âŠ¢a A â‰¤ H â‡ B
  â†’ H ~â‡§~ n
  â†’ (nâ‰¤l : n â‰¤n length Î“)
  â†’ Î“ â†“ n [ nâ‰¤l ] âŠ¢a A â‰¤ (H â‡© n) â‡ B
  
âŠ¢a-strengthen : âˆ€ {Î“ A H n e}
  â†’ Î“ âŠ¢a H â‡› e â‡› A -- H, e is shifted
  â†’ e ~â†‘~ n
  â†’ H ~â‡§~ n
  â†’ (nâ‰¤l : n â‰¤n length Î“)
  â†’ Î“ â†“ n [ nâ‰¤l ] âŠ¢a (H â‡© n) â‡› e â†“ n â‡› A

â‰¤a-strengthen â‰¤a-int sdh nâ‰¤l = â‰¤a-int
â‰¤a-strengthen â‰¤a-base sdh nâ‰¤l = â‰¤a-base
â‰¤a-strengthen â‰¤a-top sdh nâ‰¤l = â‰¤a-top
â‰¤a-strengthen â‰¤a-â–¡ sdh nâ‰¤l = â‰¤a-â–¡
â‰¤a-strengthen (â‰¤a-arr Aâ‰¤H Aâ‰¤Hâ‚) sdh nâ‰¤l = â‰¤a-arr (â‰¤a-strengthen Aâ‰¤H sdh-Ï„ nâ‰¤l) (â‰¤a-strengthen Aâ‰¤Hâ‚ sdh-Ï„ nâ‰¤l)
â‰¤a-strengthen (â‰¤a-hint âŠ¢e Aâ‰¤H) (sdh-h sd sdh) nâ‰¤l = â‰¤a-hint (âŠ¢a-strengthen âŠ¢e sd sdh-Ï„ nâ‰¤l) (â‰¤a-strengthen Aâ‰¤H sdh nâ‰¤l)
â‰¤a-strengthen (â‰¤a-and-l xâ‚ Hâ‰¢â–¡) x nâ‰¤l = â‰¤a-and-l (â‰¤a-strengthen xâ‚ x nâ‰¤l) (Hâ‰¢â–¡-â‡© Hâ‰¢â–¡)
â‰¤a-strengthen (â‰¤a-and-r xâ‚ Hâ‰¢â–¡) x nâ‰¤l = â‰¤a-and-r (â‰¤a-strengthen xâ‚ x nâ‰¤l) (Hâ‰¢â–¡-â‡© Hâ‰¢â–¡)
â‰¤a-strengthen (â‰¤a-and xâ‚ xâ‚‚) x nâ‰¤l = â‰¤a-and (â‰¤a-strengthen xâ‚ sdh-Ï„ nâ‰¤l) (â‰¤a-strengthen xâ‚‚ sdh-Ï„ nâ‰¤l)
â‰¤a-strengthen (â‰¤a-rcd xâ‚) x nâ‰¤l = {!!}
â‰¤a-strengthen (â‰¤a-hint-l xâ‚) x nâ‰¤l = {!!}

âŠ¢a-strengthen âŠ¢a-lit sd sdh nâ‰¤l = âŠ¢a-lit
âŠ¢a-strengthen (âŠ¢a-var xâˆˆÎ“) sd sdh nâ‰¤l = âŠ¢a-var (âˆ‹-strenghthen xâˆˆÎ“ sd nâ‰¤l)
âŠ¢a-strengthen (âŠ¢a-app âŠ¢e) (sd-app sdâ‚ sdâ‚‚) sdh nâ‰¤l = âŠ¢a-app (âŠ¢a-strengthen âŠ¢e sdâ‚ (sdh-h sdâ‚‚ sdh) nâ‰¤l)
âŠ¢a-strengthen (âŠ¢a-ann âŠ¢e) (sd-ann sd) sdh nâ‰¤l = âŠ¢a-ann (âŠ¢a-strengthen âŠ¢e sd sdh-Ï„ nâ‰¤l)
âŠ¢a-strengthen (âŠ¢a-lamâ‚ âŠ¢e) (sd-lam sd) sdh nâ‰¤l = âŠ¢a-lamâ‚ (âŠ¢a-strengthen âŠ¢e sd sdh-Ï„ (sâ‰¤s nâ‰¤l))
âŠ¢a-strengthen {H = âŸ¦ _ âŸ§â‡’ H} {n = n} (âŠ¢a-lamâ‚‚ âŠ¢e âŠ¢f) (sd-lam sdâ‚) (sdh-h sdâ‚‚ sdh) nâ‰¤l with âŠ¢a-strengthen âŠ¢f sdâ‚ (â‡§-shiftedh-n zâ‰¤n sdh) (sâ‰¤s nâ‰¤l)
... | ind-f rewrite sym (â‡©-â‡§-comm H 0 n zâ‰¤n sdh) = âŠ¢a-lamâ‚‚ (âŠ¢a-strengthen âŠ¢e sdâ‚‚ sdh-â–¡ nâ‰¤l) ind-f
âŠ¢a-strengthen (âŠ¢a-sub pv âŠ¢e Aâ‰¤H) sd sdh nâ‰¤l = âŠ¢a-sub (â†“-pv-prv pv) (âŠ¢a-strengthen âŠ¢e sd sdh-â–¡ nâ‰¤l) (â‰¤a-strengthen Aâ‰¤H sdh nâ‰¤l)
âŠ¢a-strengthen (âŠ¢a-& âŠ¢eâ‚ âŠ¢eâ‚‚) sd sdh nâ‰¤l = âŠ¢a-& (âŠ¢a-strengthen âŠ¢eâ‚ sd sdh-Ï„ nâ‰¤l) (âŠ¢a-strengthen âŠ¢eâ‚‚ sd sdh-Ï„ nâ‰¤l)
âŠ¢a-strengthen {e = ğ•£ xâ‚‚} (âŠ¢a-rcd xâ‚ƒ) x xâ‚ nâ‰¤l = {!!}
âŠ¢a-strengthen {e = e ğ•¡ xâ‚‚} (âŠ¢a-prj xâ‚ƒ) x xâ‚ nâ‰¤l = {!!}

â‰¤a-strengthen-0 : âˆ€ {Î“ A B C H}
  â†’ Î“ , A âŠ¢a B â‰¤ H â‡§ 0 â‡ C
  â†’ Î“ âŠ¢a B â‰¤ H â‡ C
â‰¤a-strengthen-0 {H = H} Bâ‰¤H with â‰¤a-strengthen {n = 0} Bâ‰¤H â‡§-shiftedh zâ‰¤n
... | ind-h rewrite â‡§-â‡©-id H 0 = ind-h  

âŠ¢a-strengthen-0 : âˆ€ {Î“ H e A B}
  â†’ Î“ , A âŠ¢a H â‡§ 0 â‡› e â†‘ 0 â‡› B
  â†’ Î“ âŠ¢a H â‡› e â‡› B
âŠ¢a-strengthen-0 {H = H} {e = e} âŠ¢e with âŠ¢a-strengthen {n = 0} âŠ¢e â†‘-shifted â‡§-shiftedh zâ‰¤n
... | ind-e rewrite â†‘-â†“-id e 0 | â‡§-â‡©-id H 0  = ind-e


----------------------------------------------------------------------
--+                                                                +--
--+                      General Subsumption                       +--
--+                                                                +--
----------------------------------------------------------------------
â‰¤a-refined : âˆ€ {Î“ A B H}
  â†’ Î“ âŠ¢a A â‰¤ H â‡ B
  â†’ Î“ âŠ¢a B â‰¤ H â‡ B
â‰¤a-refined â‰¤a-int = â‰¤a-int
â‰¤a-refined â‰¤a-base = â‰¤a-base
â‰¤a-refined â‰¤a-top = â‰¤a-top
â‰¤a-refined â‰¤a-â–¡ = â‰¤a-â–¡
â‰¤a-refined (â‰¤a-arr Aâ‰¤H Aâ‰¤Hâ‚) = â‰¤a-arr â‰¤a-refl (â‰¤a-refined Aâ‰¤Hâ‚)
â‰¤a-refined (â‰¤a-hint x Aâ‰¤H) = â‰¤a-hint x (â‰¤a-refined Aâ‰¤H)
â‰¤a-refined (â‰¤a-and-l Aâ‰¤H Hâ‰¢â–¡) = â‰¤a-refined Aâ‰¤H
â‰¤a-refined (â‰¤a-and-r Aâ‰¤H Hâ‰¢â–¡) = â‰¤a-refined Aâ‰¤H
â‰¤a-refined (â‰¤a-and Aâ‰¤H Aâ‰¤Hâ‚) = â‰¤a-and (â‰¤a-and-l (â‰¤a-refined Aâ‰¤H) Î» ()) (â‰¤a-and-r (â‰¤a-refined Aâ‰¤Hâ‚) Î» ())
â‰¤a-refined (â‰¤a-rcd x) = â‰¤a-rcd (â‰¤a-refined x)
â‰¤a-refined (â‰¤a-hint-l x) = â‰¤a-hint-l (â‰¤a-refined x)
