module Record.Decl.Properties where

open import Record.Prelude
open import Record.Common
open import Record.Decl
open import Record.Properties

----------------------------------------------------------------------
--+                                                                +--
--+                           Weakening                            +--
--+                                                                +--
----------------------------------------------------------------------

âŠ¢d-weaken : âˆ€ {Î“ cc e A B n}
  â†’ Î“ âŠ¢d cc # e â¦‚ B
  â†’ (nâ‰¤l : n â‰¤ length Î“)
  â†’ Î“ â†‘ n [ nâ‰¤l ] A âŠ¢d cc # (e â†‘ n) â¦‚ B

âŠ¢r-weaken : âˆ€ {Î“ rs A B n}
  â†’ Î“ âŠ¢r ğ•« # rs â¦‚ B
  â†’ (nâ‰¤l : n â‰¤ length Î“)
  â†’ Î“ â†‘ n [ nâ‰¤l ] A âŠ¢r ğ•« # (rs â†‘r n) â¦‚ B

âŠ¢d-weaken âŠ¢d-c nâ‰¤l = âŠ¢d-c
âŠ¢d-weaken (âŠ¢d-var xâˆˆÎ“) nâ‰¤l = âŠ¢d-var (âˆ‹-weaken xâˆˆÎ“ nâ‰¤l)
âŠ¢d-weaken (âŠ¢d-lamâ‚ âŠ¢e) nâ‰¤l = âŠ¢d-lamâ‚ (âŠ¢d-weaken âŠ¢e (sâ‰¤s nâ‰¤l))
âŠ¢d-weaken (âŠ¢d-lamâ‚‚ âŠ¢e) nâ‰¤l = âŠ¢d-lamâ‚‚ (âŠ¢d-weaken âŠ¢e (sâ‰¤s nâ‰¤l))
âŠ¢d-weaken (âŠ¢d-appâ‡ âŠ¢f âŠ¢e) nâ‰¤l = âŠ¢d-appâ‡ (âŠ¢d-weaken âŠ¢f nâ‰¤l) (âŠ¢d-weaken âŠ¢e nâ‰¤l)
âŠ¢d-weaken (âŠ¢d-appâ‡’ âŠ¢f âŠ¢e) nâ‰¤l = âŠ¢d-appâ‡’ (âŠ¢d-weaken âŠ¢f nâ‰¤l) (âŠ¢d-weaken âŠ¢e nâ‰¤l)
âŠ¢d-weaken (âŠ¢d-appâˆ âŠ¢f âŠ¢e) nâ‰¤l = âŠ¢d-appâˆ (âŠ¢d-weaken âŠ¢f nâ‰¤l) (âŠ¢d-weaken âŠ¢e nâ‰¤l)
-- âŠ¢d-weaken (âŠ¢d-appâˆâˆ âŠ¢f âŠ¢e) nâ‰¤l = âŠ¢d-appâˆâˆ (âŠ¢d-weaken âŠ¢f nâ‰¤l) (âŠ¢d-weaken âŠ¢e nâ‰¤l)
âŠ¢d-weaken (âŠ¢d-ann âŠ¢e) nâ‰¤l = âŠ¢d-ann (âŠ¢d-weaken âŠ¢e nâ‰¤l)
âŠ¢d-weaken (âŠ¢d-& âŠ¢eâ‚ âŠ¢eâ‚‚) nâ‰¤l = âŠ¢d-& (âŠ¢d-weaken âŠ¢eâ‚ nâ‰¤l) (âŠ¢d-weaken âŠ¢eâ‚‚ nâ‰¤l)
âŠ¢d-weaken (âŠ¢d-sub âŠ¢e Aâ‰¤B neq) nâ‰¤l = âŠ¢d-sub (âŠ¢d-weaken âŠ¢e nâ‰¤l) Aâ‰¤B neq
âŠ¢d-weaken (âŠ¢d-rcd âŠ¢e) nâ‰¤l = âŠ¢d-rcd (âŠ¢r-weaken âŠ¢e nâ‰¤l)
âŠ¢d-weaken (âŠ¢d-prj âŠ¢e) nâ‰¤l = âŠ¢d-prj (âŠ¢d-weaken âŠ¢e nâ‰¤l)
âŠ¢d-weaken (âŠ¢d-prjâˆ âŠ¢e) nâ‰¤l = âŠ¢d-prjâˆ (âŠ¢d-weaken âŠ¢e nâ‰¤l)

âŠ¢r-weaken âŠ¢r-nil nâ‰¤l = âŠ¢r-nil
âŠ¢r-weaken (âŠ¢r-one x) nâ‰¤l = âŠ¢r-one (âŠ¢d-weaken x nâ‰¤l)
âŠ¢r-weaken (âŠ¢r-cons x âŠ¢rs) nâ‰¤l = âŠ¢r-cons (âŠ¢d-weaken x nâ‰¤l) (âŠ¢r-weaken âŠ¢rs nâ‰¤l)

âŠ¢d-weaken-0 : âˆ€ {Î“ cc e A B}
  â†’ Î“ âŠ¢d cc # e â¦‚ B
  â†’ Î“ , A âŠ¢d cc # e â†‘ 0 â¦‚ B
âŠ¢d-weaken-0 âŠ¢e = âŠ¢d-weaken âŠ¢e zâ‰¤n  

----------------------------------------------------------------------
--+                                                                +--
--+                         Strengthening                          +--
--+                                                                +--
----------------------------------------------------------------------

âŠ¢d-strengthen : âˆ€ {Î“ cc e A n}
  â†’ Î“ âŠ¢d cc # e â¦‚ A
  â†’ e ~â†‘~ n
  â†’ (nâ‰¤l : n â‰¤ length Î“)
  â†’ Î“ â†“ n [ nâ‰¤l ] âŠ¢d cc # e â†“ n â¦‚ A
  
âŠ¢r-strengthen : âˆ€ {Î“ rs A n}
  â†’ Î“ âŠ¢r ğ•« # rs â¦‚ A
  â†’ rs ~â†‘r~ n
  â†’ (nâ‰¤l : n â‰¤ length Î“)
  â†’ Î“ â†“ n [ nâ‰¤l ] âŠ¢r ğ•« # rs â†“r n â¦‚ A
  
âŠ¢d-strengthen âŠ¢d-c sd nâ‰¤l = âŠ¢d-c
âŠ¢d-strengthen (âŠ¢d-var xâˆˆÎ“) sd nâ‰¤l = âŠ¢d-var (âˆ‹-strenghthen xâˆˆÎ“ sd nâ‰¤l)
âŠ¢d-strengthen (âŠ¢d-lamâ‚ âŠ¢e) (sd-lam sd) nâ‰¤l = âŠ¢d-lamâ‚ (âŠ¢d-strengthen âŠ¢e sd (sâ‰¤s nâ‰¤l))
âŠ¢d-strengthen (âŠ¢d-lamâ‚‚ âŠ¢e) (sd-lam sd) nâ‰¤l = âŠ¢d-lamâ‚‚ (âŠ¢d-strengthen âŠ¢e sd (sâ‰¤s nâ‰¤l))
âŠ¢d-strengthen (âŠ¢d-appâ‡ âŠ¢f âŠ¢e) (sd-app sd sdâ‚) nâ‰¤l = âŠ¢d-appâ‡ (âŠ¢d-strengthen âŠ¢f sd nâ‰¤l) (âŠ¢d-strengthen âŠ¢e sdâ‚ nâ‰¤l)
âŠ¢d-strengthen (âŠ¢d-appâ‡’ âŠ¢f âŠ¢e) (sd-app sd sdâ‚) nâ‰¤l = âŠ¢d-appâ‡’ (âŠ¢d-strengthen âŠ¢f sd nâ‰¤l) (âŠ¢d-strengthen âŠ¢e sdâ‚ nâ‰¤l)
âŠ¢d-strengthen (âŠ¢d-appâˆ âŠ¢f âŠ¢e) (sd-app sd sdâ‚) nâ‰¤l = âŠ¢d-appâˆ (âŠ¢d-strengthen âŠ¢f sd nâ‰¤l) (âŠ¢d-strengthen âŠ¢e sdâ‚ nâ‰¤l)
-- âŠ¢d-strengthen (âŠ¢d-appâˆâˆ âŠ¢f âŠ¢e) (sd-app sd sdâ‚) nâ‰¤l = âŠ¢d-appâˆâˆ (âŠ¢d-strengthen âŠ¢f sd nâ‰¤l) (âŠ¢d-strengthen âŠ¢e sdâ‚ nâ‰¤l)
âŠ¢d-strengthen (âŠ¢d-ann âŠ¢e) (sd-ann sd) nâ‰¤l = âŠ¢d-ann (âŠ¢d-strengthen âŠ¢e sd nâ‰¤l)
âŠ¢d-strengthen (âŠ¢d-& âŠ¢eâ‚ âŠ¢eâ‚‚) sd nâ‰¤l = âŠ¢d-& (âŠ¢d-strengthen âŠ¢eâ‚ sd nâ‰¤l) (âŠ¢d-strengthen âŠ¢eâ‚‚ sd nâ‰¤l)
âŠ¢d-strengthen (âŠ¢d-sub âŠ¢e Aâ‰¤B neq) sd nâ‰¤l = âŠ¢d-sub (âŠ¢d-strengthen âŠ¢e sd nâ‰¤l) Aâ‰¤B neq
âŠ¢d-strengthen (âŠ¢d-rcd âŠ¢e) (sd-rcd x) nâ‰¤l = âŠ¢d-rcd (âŠ¢r-strengthen âŠ¢e x nâ‰¤l)
âŠ¢d-strengthen (âŠ¢d-prj âŠ¢e) (sd-prj sd) nâ‰¤l = âŠ¢d-prj (âŠ¢d-strengthen âŠ¢e sd nâ‰¤l)
âŠ¢d-strengthen (âŠ¢d-prjâˆ âŠ¢e) (sd-prj sd) nâ‰¤l = âŠ¢d-prjâˆ (âŠ¢d-strengthen âŠ¢e sd nâ‰¤l)

âŠ¢r-strengthen âŠ¢r-nil rs~n nâ‰¤l = âŠ¢r-nil
âŠ¢r-strengthen (âŠ¢r-one x) (sdr-cons xâ‚ rs~n) nâ‰¤l = âŠ¢r-one (âŠ¢d-strengthen x xâ‚ nâ‰¤l)
âŠ¢r-strengthen (âŠ¢r-cons x âŠ¢rs) (sdr-cons xâ‚ rs~n) nâ‰¤l = âŠ¢r-cons (âŠ¢d-strengthen x xâ‚ nâ‰¤l) (âŠ¢r-strengthen âŠ¢rs rs~n nâ‰¤l)

âŠ¢d-strengthen-0 : âˆ€ {Î“ cc e A B}
  â†’ Î“ , A âŠ¢d cc # e â†‘ 0 â¦‚ B
  â†’ Î“ âŠ¢d cc # e â¦‚ B
âŠ¢d-strengthen-0 {e = e} âŠ¢e with âŠ¢d-strengthen âŠ¢e â†‘-shifted zâ‰¤n
... | ind-e rewrite â†‘-â†“-id e 0 = ind-e


âˆ‹-determinism : âˆ€ {Î“ x A B}
  â†’ Î“ âˆ‹ x â¦‚ A
  â†’ Î“ âˆ‹ x â¦‚ B
  â†’ A â‰¡ B
âˆ‹-determinism Z Z = refl
âˆ‹-determinism (S âˆ‹1) (S âˆ‹2) = âˆ‹-determinism âˆ‹1 âˆ‹2

data _â†ª_âª_,_â« : Type â†’ â„• â†’ List Type â†’ Type â†’ Set where

  n-none : âˆ€ {A}
    â†’ A â†ª 0 âª [] , A â«

  n-cons : âˆ€ {A B T n Bs}
    â†’ B â†ª n âª Bs , T â«
    â†’ (A â‡’ B) â†ª (suc n) âª A âˆ· Bs , T â«

{-

determinism is not intended

âŠ¢d-determinism : âˆ€ {Î“ e A B n As Bs Tâ‚ Tâ‚‚}
  â†’ Î“ âŠ¢d c n # e â¦‚ A
  â†’ A â†ª n âª As , Tâ‚ â«
  â†’ Î“ âŠ¢d c n # e â¦‚ B
  â†’ B â†ª n âª Bs , Tâ‚‚ â«
  â†’ As â‰¡ Bs
  â†’ Tâ‚ â‰¡ Tâ‚‚
âŠ¢d-determinism âŠ¢d-int n-none âŠ¢d-int n-none refl = refl
âŠ¢d-determinism âŠ¢d-int n-none (âŠ¢d-sub âŠ¢2 x xâ‚) n-none refl = {!!} -- done
âŠ¢d-determinism (âŠ¢d-var x) â†ª1 âŠ¢2 â†ª2 eq = {!!} -- done

âŠ¢d-determinism (âŠ¢d-lamâ‚‚ âŠ¢1) (n-cons â†ª1) (âŠ¢d-lamâ‚‚ âŠ¢2) (n-cons â†ª2) refl = âŠ¢d-determinism âŠ¢1 â†ª1 âŠ¢2 â†ª2 refl
âŠ¢d-determinism (âŠ¢d-lamâ‚‚ âŠ¢1) â†ª1 (âŠ¢d-sub âŠ¢2 x xâ‚) â†ª2 eq = {!!} -- âŠ¢2 is absurd

âŠ¢d-determinism (âŠ¢d-appâ‚ âŠ¢1 âŠ¢3) n-none (âŠ¢d-appâ‚ âŠ¢2 âŠ¢4) n-none refl = {!âŠ¢d-determinism âŠ¢1 n-none âŠ¢2 n-none refl!} -- easy
âŠ¢d-determinism (âŠ¢d-appâ‚ âŠ¢1 âŠ¢3) n-none (âŠ¢d-appâ‚‚ âŠ¢2 âŠ¢4) n-none refl = {!!} -- 
âŠ¢d-determinism (âŠ¢d-appâ‚ âŠ¢1 âŠ¢3) n-none (âŠ¢d-sub âŠ¢2 x xâ‚) n-none refl = {!!} -- absurd

âŠ¢d-determinism (âŠ¢d-appâ‚‚ âŠ¢1 âŠ¢3) â†ª1 âŠ¢2 â†ª2 eq = {!!}
âŠ¢d-determinism (âŠ¢d-ann âŠ¢1) â†ª1 âŠ¢2 â†ª2 eq = {!!}
âŠ¢d-determinism (âŠ¢d-sub âŠ¢1 x xâ‚) â†ª1 âŠ¢2 â†ª2 eq = {!!}

-}


â‰¤d-trans : âˆ€ {A B C j}
  â†’ A â‰¤d j # B
  â†’ B â‰¤d j # C
  â†’ A â‰¤d j # C
â‰¤d-trans {B = Int} â‰¤d-Z â‰¤d-Z = â‰¤d-Z
â‰¤d-trans {B = Int} â‰¤d-intâˆ â‰¤2 = â‰¤2
â‰¤d-trans {B = Int} (â‰¤d-andâ‚ â‰¤1 neq) â‰¤2 = â‰¤d-andâ‚ (â‰¤d-trans â‰¤1 â‰¤2) neq
â‰¤d-trans {B = Int} (â‰¤d-andâ‚‚ â‰¤1 neq) â‰¤2 = â‰¤d-andâ‚‚ (â‰¤d-trans â‰¤1 â‰¤2) neq
â‰¤d-trans {B = Float} â‰¤d-Z â‰¤d-Z = â‰¤d-Z
â‰¤d-trans {B = Float} â‰¤d-floatâˆ â‰¤2 = â‰¤2
â‰¤d-trans {B = Float} (â‰¤d-andâ‚ â‰¤1 neq) â‰¤2 = â‰¤d-andâ‚ (â‰¤d-trans â‰¤1 â‰¤2) neq
â‰¤d-trans {B = Float} (â‰¤d-andâ‚‚ â‰¤1 neq) â‰¤2 = â‰¤d-andâ‚‚ (â‰¤d-trans â‰¤1 â‰¤2) neq
â‰¤d-trans {B = * x} â‰¤d-Z â‰¤d-Z = â‰¤d-Z
â‰¤d-trans {B = * x} â‰¤d-baseâˆ â‰¤2 = â‰¤2
â‰¤d-trans {B = * x} (â‰¤d-andâ‚ â‰¤1 neq) â‰¤2 = â‰¤d-andâ‚ (â‰¤d-trans â‰¤1 â‰¤2) neq
â‰¤d-trans {B = * x} (â‰¤d-andâ‚‚ â‰¤1 neq) â‰¤2 = â‰¤d-andâ‚‚ (â‰¤d-trans â‰¤1 â‰¤2) neq
â‰¤d-trans {B = Top} â‰¤d-Z â‰¤d-Z = â‰¤d-Z
â‰¤d-trans {B = Top} â‰¤d-top â‰¤d-top = â‰¤d-top
â‰¤d-trans {B = Top} â‰¤d-top (â‰¤d-and â‰¤2 â‰¤3) = â‰¤d-and (â‰¤d-trans â‰¤d-top â‰¤2) (â‰¤d-trans â‰¤d-top â‰¤3)
â‰¤d-trans {B = Top} (â‰¤d-andâ‚ â‰¤1 neq) â‰¤2 = â‰¤d-andâ‚ (â‰¤d-trans â‰¤1 â‰¤2) neq
â‰¤d-trans {B = Top} (â‰¤d-andâ‚‚ â‰¤1 neq) â‰¤2 = â‰¤d-andâ‚‚ (â‰¤d-trans â‰¤1 â‰¤2) neq

â‰¤d-trans {B = B â‡’ Bâ‚} â‰¤d-Z â‰¤2 = â‰¤2
â‰¤d-trans {B = B â‡’ Bâ‚} (â‰¤d-arr-âˆ â‰¤1 â‰¤3) â‰¤d-top = â‰¤d-top
â‰¤d-trans {B = B â‡’ Bâ‚} (â‰¤d-arr-âˆ â‰¤1 â‰¤3) (â‰¤d-arr-âˆ â‰¤2 â‰¤4) = â‰¤d-arr-âˆ (â‰¤d-trans â‰¤2 â‰¤1) (â‰¤d-trans â‰¤3 â‰¤4)
â‰¤d-trans {B = B â‡’ Bâ‚} (â‰¤d-arr-âˆ â‰¤1 â‰¤3) (â‰¤d-and â‰¤2 â‰¤4) = â‰¤d-and (â‰¤d-trans (â‰¤d-arr-âˆ â‰¤1 â‰¤3) â‰¤2) (â‰¤d-trans (â‰¤d-arr-âˆ â‰¤1 â‰¤3) â‰¤4)
â‰¤d-trans {B = B â‡’ Bâ‚} (â‰¤d-arr-Sâ‡ â‰¤1 â‰¤3) (â‰¤d-arr-Sâ‡ â‰¤2 â‰¤4) = â‰¤d-arr-Sâ‡ â‰¤2 (â‰¤d-trans â‰¤3 â‰¤4)

â‰¤d-trans {B = B â‡’ Bâ‚} (â‰¤d-andâ‚ â‰¤1 neq) â‰¤2 = â‰¤d-andâ‚ (â‰¤d-trans â‰¤1 â‰¤2) neq
â‰¤d-trans {B = B â‡’ Bâ‚} (â‰¤d-andâ‚‚ â‰¤1 neq) â‰¤2 = â‰¤d-andâ‚‚ (â‰¤d-trans â‰¤1 â‰¤2) neq
â‰¤d-trans {B = B & Bâ‚} â‰¤d-Z â‰¤2 = â‰¤2
â‰¤d-trans {B = B & Bâ‚} (â‰¤d-andâ‚ â‰¤1 neq) â‰¤2 = â‰¤d-andâ‚ (â‰¤d-trans â‰¤1 â‰¤2) neq
â‰¤d-trans {B = B & Bâ‚} (â‰¤d-andâ‚‚ â‰¤1 neq) â‰¤2 = â‰¤d-andâ‚‚ (â‰¤d-trans â‰¤1 â‰¤2) neq
â‰¤d-trans {B = B & Bâ‚} (â‰¤d-and â‰¤1 â‰¤3) â‰¤d-top = â‰¤d-top
â‰¤d-trans {B = B & Bâ‚} (â‰¤d-and â‰¤1 â‰¤3) (â‰¤d-andâ‚ â‰¤2 neq) = â‰¤d-trans â‰¤1 â‰¤2
â‰¤d-trans {B = B & Bâ‚} (â‰¤d-and â‰¤1 â‰¤3) (â‰¤d-andâ‚‚ â‰¤2 neq) = â‰¤d-trans â‰¤3 â‰¤2
â‰¤d-trans {B = B & Bâ‚} (â‰¤d-and â‰¤1 â‰¤3) (â‰¤d-and â‰¤2 â‰¤4) = â‰¤d-and (â‰¤d-trans (â‰¤d-and â‰¤1 â‰¤3) â‰¤2) (â‰¤d-trans (â‰¤d-and â‰¤1 â‰¤3) â‰¤4)

â‰¤d-trans {B = Ï„âŸ¦ l â†¦ B âŸ§} â‰¤d-Z â‰¤2 = â‰¤2
â‰¤d-trans {B = Ï„âŸ¦ l â†¦ B âŸ§} (â‰¤d-rcdâˆ â‰¤1) â‰¤d-top = â‰¤d-top
â‰¤d-trans {B = Ï„âŸ¦ l â†¦ B âŸ§} (â‰¤d-rcdâˆ â‰¤1) (â‰¤d-rcdâˆ â‰¤2) = â‰¤d-rcdâˆ (â‰¤d-trans â‰¤1 â‰¤2)
â‰¤d-trans {B = Ï„âŸ¦ l â†¦ B âŸ§} (â‰¤d-rcdâˆ â‰¤1) (â‰¤d-and â‰¤2 â‰¤3) = â‰¤d-and (â‰¤d-trans (â‰¤d-rcdâˆ â‰¤1) â‰¤2) (â‰¤d-trans (â‰¤d-rcdâˆ â‰¤1) â‰¤3)
â‰¤d-trans {B = Ï„âŸ¦ l â†¦ B âŸ§} (â‰¤d-rcd-Sl â‰¤1) (â‰¤d-rcd-Sl â‰¤2) = â‰¤d-rcd-Sl (â‰¤d-trans â‰¤1 â‰¤2)
â‰¤d-trans {B = Ï„âŸ¦ l â†¦ B âŸ§} (â‰¤d-andâ‚ â‰¤1 neq) â‰¤2 = â‰¤d-andâ‚ (â‰¤d-trans â‰¤1 â‰¤2) neq
â‰¤d-trans {B = Ï„âŸ¦ l â†¦ B âŸ§} (â‰¤d-andâ‚‚ â‰¤1 neq) â‰¤2 = â‰¤d-andâ‚‚ (â‰¤d-trans â‰¤1 â‰¤2) neq

----------------------------------------------------------------------
--+                                                                +--
--+                           Subsumption                          +--
--+                                                                +--
----------------------------------------------------------------------

âŠ¢d-sub' : âˆ€ {Î“ e A B i}
  â†’ Î“ âŠ¢d ğ•« # e â¦‚ B
  â†’ B â‰¤d i # A
  â†’ Î“ âŠ¢d i # e â¦‚ A
âŠ¢d-sub' {i = ğ•š (ğ•“ Z)} âŠ¢e â‰¤d-Z = âŠ¢e
âŠ¢d-sub' {i = ğ•š (ğ•“ Z)} âŠ¢e (â‰¤d-andâ‚ Bâ‰¤A x) = âŠ¥-elim (x refl)
âŠ¢d-sub' {i = ğ•š (ğ•“ Z)} âŠ¢e (â‰¤d-andâ‚‚ Bâ‰¤A x) = âŠ¥-elim (x refl)
âŠ¢d-sub' {i = ğ•š (ğ•“ (Sâ‡ j))} âŠ¢e Bâ‰¤A = âŠ¢d-sub âŠ¢e Bâ‰¤A (Î» ())
âŠ¢d-sub' {i = ğ•š (ğ•“ (Sl j))} âŠ¢e Bâ‰¤A = âŠ¢d-sub âŠ¢e Bâ‰¤A (Î» ())
âŠ¢d-sub' {i = ğ•š (Sâ‡’ i)} âŠ¢e Bâ‰¤A = âŠ¢d-sub âŠ¢e Bâ‰¤A (Î» ())
âŠ¢d-sub' {i = âˆ} âŠ¢e Bâ‰¤A = âŠ¢d-sub âŠ¢e Bâ‰¤A (Î» ())
