module Record.Common where

open import Record.Prelude hiding (_â‰¤?_)

  
Id : Set
Id = String

infixr 5  Æ›_
infixl 7  _Â·_
infix  9  `_
infix  5  _â¦‚_
infixr 8 _â‡’_
-- infixr 8 _&_
infix  2 ğ•£_
infixr 5 râŸ¦_â†¦_âŸ§_

infix 9 *_ 
Label = â„•

data Type : Set where
  Int : Type
  Float : Type
  *_ : â„• â†’ Type
  Top : Type
  _â‡’_ : Type â†’ Type â†’ Type
  _&_ : Type â†’ Type â†’ Type
  Ï„âŸ¦_â†¦_âŸ§ : Label â†’ Type â†’ Type

data Constant : Set where
  lit      : â„• â†’ Constant
  flt      : ğ”½ â†’ Constant
  +s       : Constant
  +i       : â„• â†’ Constant
  +f       : ğ”½ â†’ Constant

data Term : Set
data Record : Set

data Term where
  ğ•”_       : Constant â†’ Term
  `_       : â„• â†’ Term
  Æ›_       : Term â†’ Term
  _Â·_      : Term â†’ Term â†’ Term
  _â¦‚_      : Term â†’ Type â†’ Term
  ğ•£_       : Record â†’ Term
  _ğ•¡_      : Term â†’ Label â†’ Term

data Record where
  rnil : Record
  râŸ¦_â†¦_âŸ§_ : Label â†’ Term â†’ Record â†’ Record

c-Ï„ : Constant â†’ Type
c-Ï„ (lit n) = Int
c-Ï„ (flt n) = Float
c-Ï„ +s = (Int â‡’ Int â‡’ Int) & (Float â‡’ Float â‡’ Float)
c-Ï„ (+i n) = Int â‡’ Int
c-Ï„ (+f n) = Float â‡’ Float

infixl 5  _,_

data Context : Set where
  âˆ…     : Context
  _,_   : Context â†’ Type â†’ Context

infix  4  _âˆ‹_â¦‚_

data _âˆ‹_â¦‚_ : Context â†’ â„• â†’ Type â†’ Set where

  Z : âˆ€ {Î“ A}
      ------------------
    â†’ Î“ , A âˆ‹ zero â¦‚ A

  S : âˆ€ {Î“ A B n}
    â†’ Î“ âˆ‹ n â¦‚ A
      ------------------
    â†’ Î“ , B âˆ‹ (suc n) â¦‚ A

----------------------------------------------------------------------
--+                                                                +--
--+                             Shift                              +--
--+                                                                +--
----------------------------------------------------------------------
abstract
  _â‰¤?_ : (x y : â„•) â†’ Dec (x â‰¤ y)
  _â‰¤?_ = Record.Prelude._â‰¤?_

â†‘-var : â„• â†’ â„• â†’ â„•
â†‘-var n x with n â‰¤? x
... | yes nâ‰¤x = suc x
... | no  n>x = x

infixl 7 _â†‘_
infixl 7 _â†‘r_
_â†‘_ : Term â†’ â„• â†’ Term
_â†‘r_ : Record â†’ â„• â†’ Record

(ğ•” c) â†‘ n = ğ•” c
` x â†‘ n = ` (â†‘-var n x)
(Æ› e) â†‘ n = Æ› (e â†‘ (suc n))
eâ‚ Â· eâ‚‚ â†‘ n = (eâ‚ â†‘ n) Â· (eâ‚‚ â†‘ n)
(e â¦‚ A) â†‘ n = (e â†‘ n) â¦‚ A
(ğ•£ rs) â†‘ n = ğ•£ (rs â†‘r n)
(e ğ•¡ l) â†‘ n = (e â†‘ n) ğ•¡ l

rnil â†‘r n = rnil
(râŸ¦ l â†¦ e âŸ§ rs) â†‘r n = râŸ¦ l â†¦ (e â†‘ n) âŸ§ (rs â†‘r n)

â†“-var : â„• â†’ â„• â†’ â„•
â†“-var n x with n â‰¤? x
... | yes nâ‰¤x = pred x
... | no n>x   = x

infixl 7 _â†“_
infixl 7 _â†“r_

_â†“_ : Term â†’ â„• â†’ Term
_â†“r_ : Record â†’ â„• â†’ Record

ğ•” c â†“ n = ğ•” c
` x â†“ n = ` (â†“-var n x)
(Æ› e) â†“ n = Æ› (e â†“ (suc n))
eâ‚ Â· eâ‚‚ â†“ n = (eâ‚ â†“ n) Â· (eâ‚‚ â†“ n)
(e â¦‚ A) â†“ n = (e â†“ n) â¦‚ A
(ğ•£ rs) â†“ n = ğ•£ (rs â†“r n)
(e ğ•¡ l) â†“ n = (e â†“ n) ğ•¡ l

rnil â†“r n = rnil
(râŸ¦ l â†¦ e âŸ§ rs) â†“r n = râŸ¦ l â†¦ (e â†“ n) âŸ§ (rs â†“r n)



â†‘-â†“-var : âˆ€ x n â†’ â†“-var n (â†‘-var n x) â‰¡ x
â†‘-â†“-var x n with n â‰¤? x
...         | yes nâ‰¤x with n â‰¤? suc x
...                   | yes nâ‰¤x+1 = refl
...                   | no  nâ‰°x+1 = âŠ¥-elim (nâ‰°x+1 (mâ‰¤nâ‡’mâ‰¤1+n nâ‰¤x))
â†‘-â†“-var x n | no  nâ‰°x with n â‰¤? x
...                   | yes nâ‰¤x = âŠ¥-elim (nâ‰°x nâ‰¤x)
...                   | no  nâ‰°x = refl


â†‘-â†“-id : âˆ€ e n
  â†’ e â†‘ n â†“ n â‰¡ e

â†‘r-â†“r-id : âˆ€ rs n
  â†’ rs â†‘r n â†“r n â‰¡ rs

â†‘-â†“-id (ğ•” _) n = refl
â†‘-â†“-id (` x) n = cong `_ (â†‘-â†“-var x n)
â†‘-â†“-id (Æ› e) n rewrite â†‘-â†“-id e (suc n) = refl
â†‘-â†“-id (eâ‚ Â· eâ‚‚) n rewrite â†‘-â†“-id eâ‚ n | â†‘-â†“-id eâ‚‚ n = refl
â†‘-â†“-id (e â¦‚ A) n rewrite â†‘-â†“-id e n = refl
â†‘-â†“-id (ğ•£ rs) n rewrite â†‘r-â†“r-id rs n = refl
â†‘-â†“-id (e ğ•¡ l) n rewrite â†‘-â†“-id e n = refl

â†‘r-â†“r-id rnil n = refl
â†‘r-â†“r-id (râŸ¦ l â†¦ e âŸ§ rs) n rewrite â†‘-â†“-id e n | â†‘r-â†“r-id rs n = refl


â†‘-â†‘-comm-var : âˆ€ m n x
  â†’ m â‰¤ n
  â†’ â†‘-var (suc n) (â†‘-var m x) â‰¡ â†‘-var m (â†‘-var n x)
â†‘-â†‘-comm-var m n x mâ‰¤n with m â‰¤? x | n â‰¤? x
...               | yes mâ‰¤x | yes nâ‰¤x with suc n â‰¤? suc x | m â‰¤? suc x
...                                   | yes n+1â‰¤x+1 | yes mâ‰¤x+1 = refl
...                                   | yes n+1â‰¤x+1 | no  mâ‰°x+1 = âŠ¥-elim (mâ‰°x+1 (mâ‰¤nâ‡’mâ‰¤1+n mâ‰¤x))
...                                   | no  n+1â‰°x+1 | yes mâ‰¤x+1 = âŠ¥-elim (n+1â‰°x+1 (sâ‰¤s nâ‰¤x))
...                                   | no  n+1â‰°x+1 | no  mâ‰°x+1 = refl
â†‘-â†‘-comm-var m n x mâ‰¤n | yes mâ‰¤x | no nâ‰°x  with suc n â‰¤? suc x | m â‰¤? x
...                                   | yes n+1â‰¤x+1 | yes mâ‰¤x = âŠ¥-elim (nâ‰°x (â‰¤-pred n+1â‰¤x+1))
...                                   | yes n+1â‰¤x+1 | no  mâ‰°x = âŠ¥-elim (mâ‰°x mâ‰¤x)
...                                   | no  n+1â‰°x+1 | yes mâ‰¤x = refl
...                                   | no  n+1â‰°x+1 | no  mâ‰°x = âŠ¥-elim (mâ‰°x mâ‰¤x)
â†‘-â†‘-comm-var m n x mâ‰¤n | no  mâ‰°x | yes nâ‰¤x with suc n â‰¤? x | m â‰¤? suc x
...                                   | yes n+1â‰¤x | yes mâ‰¤x+1 = âŠ¥-elim (mâ‰°x (â‰¤-trans mâ‰¤n nâ‰¤x))
...                                   | yes n+1â‰¤x | no  mâ‰°x+1 = refl
...                                   | no  n+1â‰°x | yes mâ‰¤x+1 = âŠ¥-elim (mâ‰°x (â‰¤-trans mâ‰¤n nâ‰¤x))
...                                   | no  n+1â‰°x | no  mâ‰°x+1 = âŠ¥-elim (mâ‰°x (â‰¤-trans mâ‰¤n nâ‰¤x))
â†‘-â†‘-comm-var m n x mâ‰¤n | no  mâ‰°x | no nâ‰°x  with suc n â‰¤? x | m â‰¤? x
...                                   | yes n+1â‰¤x | yes mâ‰¤x = refl
...                                   | yes n+1â‰¤x | no  mâ‰°x = âŠ¥-elim (nâ‰°x (m+1â‰¤nâ†’mâ‰¤n n+1â‰¤x))
...                                   | no  n+1â‰°x | yes mâ‰¤x = âŠ¥-elim (mâ‰°x mâ‰¤x)
...                                   | no  n+1â‰°x | no  mâ‰°x = refl


â†‘-â†‘-comm : âˆ€ e m n â†’ m â‰¤ n â†’ e â†‘ m â†‘ suc n â‰¡ e â†‘ n â†‘ m
â†‘r-â†‘r-comm : âˆ€ rs m n â†’ m â‰¤ n â†’ rs â†‘r m â†‘r suc n â‰¡ rs â†‘r n â†‘r m

â†‘-â†‘-comm (ğ•” _) m n mâ‰¤n = refl
â†‘-â†‘-comm (` x) m n mâ‰¤n = cong `_ (â†‘-â†‘-comm-var m n x mâ‰¤n)
â†‘-â†‘-comm (Æ› e) m n mâ‰¤n rewrite â†‘-â†‘-comm e (suc m) (suc n) (sâ‰¤s mâ‰¤n) = refl
â†‘-â†‘-comm (eâ‚ Â· eâ‚‚) m n mâ‰¤n rewrite â†‘-â†‘-comm eâ‚ m n mâ‰¤n | â†‘-â†‘-comm eâ‚‚ m n mâ‰¤n = refl
â†‘-â†‘-comm (e â¦‚ A) m n mâ‰¤n rewrite â†‘-â†‘-comm e m n mâ‰¤n = refl
â†‘-â†‘-comm (ğ•£ rs) m n mâ‰¤n rewrite â†‘r-â†‘r-comm rs m n mâ‰¤n = refl
â†‘-â†‘-comm (e ğ•¡ l) m n mâ‰¤n rewrite â†‘-â†‘-comm e m n mâ‰¤n = refl
â†‘r-â†‘r-comm rnil m n mâ‰¤n = refl
â†‘r-â†‘r-comm (râŸ¦ l â†¦ e âŸ§ rs) m n mâ‰¤n rewrite â†‘-â†‘-comm e m n mâ‰¤n | â†‘r-â†‘r-comm rs m n mâ‰¤n = refl

infix 4 _~â†‘~_
infix 4 _~â†‘r~_

data _~â†‘~_ : Term â†’ â„• â†’ Set
data _~â†‘r~_ : Record â†’ â„• â†’ Set

data _~â†‘~_ where

  sd-c : âˆ€ {n c}
    â†’ (ğ•” c) ~â†‘~ n

  sd-var : âˆ€ {n x}
    â†’ n â‰¢ x
    â†’ (` x) ~â†‘~ n

  sd-lam : âˆ€ {n e}
    â†’ e ~â†‘~ (suc n)
    â†’ (Æ› e) ~â†‘~ n

  sd-app : âˆ€ {n eâ‚ eâ‚‚}
    â†’ eâ‚ ~â†‘~ n
    â†’ eâ‚‚ ~â†‘~ n
    â†’ (eâ‚ Â· eâ‚‚) ~â†‘~ n

  sd-ann : âˆ€ {n e A}
    â†’ e ~â†‘~ n
    â†’ (e â¦‚ A) ~â†‘~ n

  sd-rcd : âˆ€ {n rs}
    â†’ rs ~â†‘r~ n
    â†’ (ğ•£ rs) ~â†‘~ n

  sd-prj : âˆ€ {e l n}
    â†’ e ~â†‘~ n
    â†’ (e ğ•¡ l) ~â†‘~ n

data _~â†‘r~_ where

  sdr-nil : âˆ€ {n}
    â†’ rnil ~â†‘r~ n

  sdr-cons : âˆ€ {e n rs l}
    â†’ e ~â†‘~ n
    â†’ rs ~â†‘r~ n
    â†’ râŸ¦ l â†¦ e âŸ§ rs ~â†‘r~ n


â†‘-shifted : âˆ€ {e n}
  â†’ (e â†‘ n) ~â†‘~ n
â†‘r-shifted : âˆ€ {rs n}
  â†’ (rs â†‘r n) ~â†‘r~ n

â†‘-shifted {ğ•” c} {n} = sd-c
â†‘-shifted {` x} {n} with n â‰¤? x
... | yes p = sd-var (<â‡’â‰¢ (sâ‰¤s p))
... | no Â¬p = sd-var (>â‡’â‰¢ (â‰°â‡’> Â¬p))
â†‘-shifted {Æ› e} {n} = sd-lam (â†‘-shifted {e})
â†‘-shifted {eâ‚ Â· eâ‚‚} {n} = sd-app (â†‘-shifted {eâ‚}) (â†‘-shifted {eâ‚‚})
â†‘-shifted {e â¦‚ A} {n} = sd-ann (â†‘-shifted {e})
â†‘-shifted {ğ•£ rs} {n} = sd-rcd â†‘r-shifted
â†‘-shifted {e ğ•¡ l} {n} = sd-prj â†‘-shifted

â†‘r-shifted {rnil} {n} = sdr-nil
â†‘r-shifted {râŸ¦ l â†¦ e âŸ§ rs} {n} = sdr-cons â†‘-shifted (â†‘r-shifted {rs})

â†“-â†‘-comm-var : âˆ€ m n x
  â†’ m â‰¤ n
  â†’ n â‰¢ x
  â†’ â†‘-var m (â†“-var n x) â‰¡ â†“-var (suc n) (â†‘-var m x)
â†“-â†‘-comm-var m n x mâ‰¤n nâ‰¢x with n â‰¤? x | m â‰¤? x
...                        | yes nâ‰¤x | yes mâ‰¤x with m â‰¤? pred x | suc n â‰¤? suc x
...                                            | yes mâ‰¤x-1 | yes n+1â‰¤x+1 = n-1+1â‰¡n+1-1 (m<nâ‡’0<n (â‰¤âˆ§â‰¢â‡’< nâ‰¤x nâ‰¢x))
...                                            | yes mâ‰¤x-1 | no  n+1â‰°x+1 = âŠ¥-elim (n+1â‰°x+1 (sâ‰¤s nâ‰¤x))
...                                            | no  mâ‰°x-1 | yes n+1â‰¤x+1 = âŠ¥-elim (mâ‰°x-1 (<â‡’â‰¤pred m<x)) where m<x = <-transÊ³ mâ‰¤n (â‰¤âˆ§â‰¢â‡’< nâ‰¤x nâ‰¢x)
...                                            | no  mâ‰°x-1 | no  n+1â‰°x+1 = âŠ¥-elim (n+1â‰°x+1 (sâ‰¤s nâ‰¤x))
â†“-â†‘-comm-var m n x mâ‰¤n nâ‰¢x | yes nâ‰¤x | no  mâ‰°x with m â‰¤? pred x | suc n â‰¤? x
...                                            | yes mâ‰¤x-1 | yes n+1â‰¤x = âŠ¥-elim (mâ‰°x (â‰¤-trans mâ‰¤n nâ‰¤x))
...                                            | yes mâ‰¤x-1 | no  n+1â‰°x = n-1+1â‰¡n+1-1 (m<nâ‡’0<n (â‰¤âˆ§â‰¢â‡’< nâ‰¤x nâ‰¢x))
...                                            | no  mâ‰°x-1 | yes n+1â‰¤x = refl
...                                            | no  mâ‰°x-1 | no  n+1â‰°x = âŠ¥-elim (n+1â‰°x (â‰¤âˆ§â‰¢â‡’< nâ‰¤x nâ‰¢x))
â†“-â†‘-comm-var m n x mâ‰¤n nâ‰¢x | no  nâ‰°x | yes mâ‰¤x with m â‰¤? x | suc n â‰¤? suc x
...                                            | yes mâ‰¤x | yes n+1â‰¤x+1 = âŠ¥-elim (nâ‰°x (â‰¤-pred n+1â‰¤x+1))
...                                            | yes mâ‰¤x | no  n+1â‰°x+1 = refl
...                                            | no  mâ‰°x | yes n+1â‰¤x+1 = refl
...                                            | no  mâ‰°x | no  n+1â‰°x+1 = âŠ¥-elim (mâ‰°x mâ‰¤x)
â†“-â†‘-comm-var m n x mâ‰¤n nâ‰¢x | no  nâ‰°x | no  mâ‰°x with m â‰¤? x | suc n â‰¤? x
...                                            | yes mâ‰¤x | yes n+1â‰¤x = âŠ¥-elim (mâ‰°x mâ‰¤x)
...                                            | yes mâ‰¤x | no  n+1â‰°x = âŠ¥-elim (mâ‰°x mâ‰¤x)
...                                            | no  mâ‰°x | yes n+1â‰¤x = âŠ¥-elim (nâ‰°x (m+1â‰¤nâ†’mâ‰¤n n+1â‰¤x))
...                                            | no  mâ‰°x | no  n+1â‰°x = refl
  

â†“-â†‘-comm : âˆ€ e m n
  â†’ m â‰¤ n
  â†’ e ~â†‘~ n
  â†’ e â†“ n â†‘ m â‰¡ e â†‘ m â†“ (suc n)
â†“r-â†‘r-comm : âˆ€ rs m n
  â†’ m â‰¤ n
  â†’ rs ~â†‘r~ n
  â†’ rs â†“r n â†‘r m â‰¡ rs â†‘r m â†“r (suc n)  
â†“-â†‘-comm (ğ•” x) m n mâ‰¤n sd = refl
â†“-â†‘-comm (` x) m n mâ‰¤n (sd-var nâ‰¢x) = cong `_ (â†“-â†‘-comm-var m n x mâ‰¤n nâ‰¢x)
â†“-â†‘-comm (Æ› e) m n mâ‰¤n (sd-lam sd) rewrite â†“-â†‘-comm e (suc m) (suc n) (sâ‰¤s mâ‰¤n) sd = refl
â†“-â†‘-comm (eâ‚ Â· eâ‚‚) m n mâ‰¤n (sd-app sdâ‚ sdâ‚‚) rewrite â†“-â†‘-comm eâ‚ m n mâ‰¤n sdâ‚ | â†“-â†‘-comm eâ‚‚ m n mâ‰¤n sdâ‚‚ = refl
â†“-â†‘-comm (e â¦‚ A) m n mâ‰¤n (sd-ann sd) rewrite â†“-â†‘-comm e m n mâ‰¤n sd = refl
â†“-â†‘-comm (ğ•£ rs) m n mâ‰¤n (sd-rcd x) rewrite â†“r-â†‘r-comm rs m n mâ‰¤n x = refl
â†“-â†‘-comm (e ğ•¡ l) m n mâ‰¤n (sd-prj sd) rewrite â†“-â†‘-comm e m n mâ‰¤n sd = refl

â†“r-â†‘r-comm rnil m n mâ‰¤n sd = refl
â†“r-â†‘r-comm (râŸ¦ l â†¦ e âŸ§ rs) m n mâ‰¤n (sdr-cons x sd) rewrite â†“-â†‘-comm e m n mâ‰¤n x | â†“r-â†‘r-comm rs m n mâ‰¤n sd = refl


â†‘-shifted-n : âˆ€ {e m n}
  â†’ m â‰¤ suc n
  â†’ e ~â†‘~ n
  â†’ (e â†‘ m) ~â†‘~ suc n
â†‘r-shifted-n : âˆ€ {rs m n}
  â†’ m â‰¤ suc n
  â†’ rs ~â†‘r~ n
  â†’ (rs â†‘r m) ~â†‘r~ suc n  
â†‘-shifted-n {ğ•” x} mâ‰¤n+1 sd = sd-c
â†‘-shifted-n {` x} {m} mâ‰¤n+1 (sd-var xâ‚) with m â‰¤? x
... | yes p = sd-var Î» n+1â‰¡x+1 â†’ xâ‚ (cong pred n+1â‰¡x+1)
... | no Â¬p = sd-var (â‰¢-sym (<â‡’â‰¢ (<-transË¡ (mâ‰°nâ‡’n<m Â¬p) mâ‰¤n+1)))
â†‘-shifted-n {Æ› e} mâ‰¤n+1 (sd-lam sd) = sd-lam (â†‘-shifted-n (sâ‰¤s mâ‰¤n+1) sd)
â†‘-shifted-n {e Â· eâ‚} mâ‰¤n+1 (sd-app sd sdâ‚) = sd-app (â†‘-shifted-n mâ‰¤n+1 sd) (â†‘-shifted-n mâ‰¤n+1 sdâ‚)
â†‘-shifted-n {e â¦‚ x} mâ‰¤n+1 (sd-ann sd) = sd-ann (â†‘-shifted-n mâ‰¤n+1 sd)
â†‘-shifted-n {ğ•£ rs} mâ‰¤n+1 (sd-rcd x) = sd-rcd (â†‘r-shifted-n mâ‰¤n+1 x)
â†‘-shifted-n {e ğ•¡ l} mâ‰¤n+1 (sd-prj sd) = sd-prj (â†‘-shifted-n mâ‰¤n+1 sd)
â†‘r-shifted-n {rnil} mâ‰¤n+1 sdr-nil = sdr-nil
â†‘r-shifted-n {râŸ¦ l â†¦ e âŸ§ rs} mâ‰¤n+1 (sdr-cons xâ‚‚ sd) = sdr-cons (â†‘-shifted-n mâ‰¤n+1 xâ‚‚) (â†‘r-shifted-n mâ‰¤n+1 sd)
